<?xml version='1.0' encoding='UTF-8'?>
<rdf:RDF xmlns:lrmoo="http://iflastandards.info/ns/lrm/lrmoo/" xmlns:owl="http://www.w3.org/2002/07/owl#" xmlns:rdf="http://www.w3.org/1999/02/22-rdf-syntax-ns#" xmlns:rdfs="http://www.w3.org/2000/01/rdf-schema#" xmlns:skos="http://www.w3.org/2004/02/skos/core#" xml:base="http://iflastandards.info/ns/lrm/lrmoo/">
  <!--
OWL implementation of LRMoo v1.0 May, 2024 (https://cidoc-crm.org/frbroo/ModelVersion/version-1.0-2)).

Created by FORTH-ICS - June, 2024
CC BY 4.0 https://creativecommons.org/licenses/by/4.0/legalcode

-->
  <owl:Ontology rdf:about="">
    <rdfs:label xml:lang="en">LRMoo 1.0 / OWL</rdfs:label>
    <owl:versionInfo xml:lang="en">LRMoo Ontology 1.0 (May, 2024) including references to CIDOC-CRM 7.1.3</owl:versionInfo>
  </owl:Ontology>
  <owl:Class rdf:about="F1_Work">
    <rdfs:label xml:lang="en">F1 Work</rdfs:label>
    <skos:notation>F1</skos:notation>
    <skos:prefLabel xml:lang="en">Work</skos:prefLabel>
    <rdfs:subClassOf rdf:resource="http://www.cidoc-crm.org/cidoc-crm/E89_Propositional_Object"/>
    <rdfs:comment xml:lang="en">Scope note:
This class comprises distinct intellectual ideas conveyed in artistic and intellectual creations, such a poems, stories or musical compositions.
A Work is the outcome of an intellectual process of one or more persons. Inherent to the notion of work is the existence of recognisable realizations of the work in the form of one or more expressions. Works are often regarded as finished and discrete e.g. when declared as such by the creator of the work or based on the elaboration or logical coherence of its content. However, works may be recognized as existing but unfinished e.g. if the creators deliberately or accidentally never explicitly finished a particular Expression but have left behind partial expressions.
In the absence of explicit information about the initial conception, which is rarely available, the first expression created constitutes witness of the beginning of existence of a Work.
A Work can evolve over time, such as through revised editions. A Work may be elaborated by one or more Actors simultaneously, in parallel, or over time. Additional expressions of a Work can continue to be created over time.
The boundaries of a Work have nothing to do with the value of the intellectual achievement but only with the dominance of a concept.
The main purpose of this class is to enable bringing together intellectually equivalent Expressions in order to display to a user all available alternatives of the same intellectual or artistic content.

Examples:
- Agatha Christie’s ‘Murder on the Orient Express’ [novel]
- Mary Shelley’s ‘Frankenstein, or, The Modern Prometheus’ [novel]
- Ursula K. Le Guin’s ‘The Earthsea trilogy’ [set of novels]
- Ursula K. Le Guin’s ‘The Tombs of Atuan’ [novel which is part of ‘The Earthsea trilogy’]
- Homer’s ‘Odyssey’ [ancient Greek epic poem]
- Dante’s ‘Divina Commedia’ [narrative poem]
- William Shakespeare’s ‘The Tragedy of Hamlet, Prince of Denmark’ [play]
- Henry Gray’s ‘Anatomy of the human body’ [scholarly work / reference work]
- René Goscinny and Albert Uderzo’s ‘Astérix le Gaulois’ [cartoon]
- the ‘Dewey Decimal Classification’ (DDC) [library classification system]
- the Ordnance Survey’s 1:50 000 ‘Landranger series’ [collection of maps]
- Ludwig van Beethoven’s ‘Symphony No. 9 in D minor’ [symphony]
- Johann Sebastian Bach’s ‘Goldberg Variations’ [compositions for keyboard]
- Daniel Humair and Damien Varaillon’s ‘Hommage à John Coltrane’ [musical improvisation]
- John Lennon and Paul McCartney’s ‘I want to hold your hand’ [song]
- François Truffault’s ‘Jules et Jim’ [movie]
- Alfred Hitchcock’s ‘Psycho’ [movie]
- Auguste Rodin’s ‘Le penseur’ (‘The thinker’) [art]
- Pablo Picasso’s ‘Guernica’ [art]
- Katsushika Hokusai’s ‘神奈川沖浪裏’ (‘The Great Wave’) [art]
</rdfs:comment>
  </owl:Class>
  <owl:Class rdf:about="F2_Expression">
    <rdfs:label xml:lang="en">F2 Expression</rdfs:label>
    <skos:notation>F2</skos:notation>
    <skos:prefLabel xml:lang="en">Expression</skos:prefLabel>
    <rdfs:subClassOf rdf:resource="http://www.cidoc-crm.org/cidoc-crm/E73_Information_Object"/>
    <rdfs:comment xml:lang="en">Scope note:
This class comprises the intellectual or artistic realisations of Works in the form of identifiable immaterial objects, such as texts, poems, jokes, musical or choreographic notations, movement pattern, sound pattern, images, multimedia objects, or any combination of such forms. The substance of F2 Expression is signs.
An Expression is the outcome of the intellectual or creative process of realizing a Work. Subsequent expressions conveying the same work may be created over time.
Expressions do not depend on a specific physical carrier and can exist on one or more carriers simultaneously. As far as bibliographic practice is concerned, only instances of F2 Expression that are externalised on physical carriers other than both the creator’s brain and an auditor’s brain are taken into account.
The form of F2 Expression is an inherent characteristic of the F2 Expression. Differences in form imply different Expressions (e.g., from text to spoken word, a transcript of a recording). Similarly, differences in language or means of performance imply different Expressions (e.g., translations or arrangements for different instruments). Thus, if a text is revised or modified, the result is considered to be a new F2 Expression. While theoretically any change in signs will result in a new Expression, conventionally the context and use will determine the rules for distinguishing among expressions.
An instance of F2 Expression which includes spoken or written text may be multiply instantiated as an instance of E33 Linguistic Object. This allows for the association of the E56 Language of the text with the instance of F2 Expression by using the property P72 has language (is language of).

Examples:
- the original text (in English) by Agatha Christie for her novel ‘Murder on the Orient Express’
- the German text of ‘Murder on the Orient Express’ (as translated by Elisabeth van Bebber and published with the title ‘Mord im Orientexpress’)
- the text of the abridged English version of ‘Murder on the Orient Express’ (as published by HarperCollins)
- the narrated English text of ‘Murder on the Orient Express’ by David Suchet
- the English text of Homer’s ‘Odyssey’ translated by Robert Fagles
- the English text of Homer’s ‘Odyssey’ translated by Richmond Lattimore
- ‘Dewey Decimal Classification’, 23rd edition (DDC23) [English edition]
- ‘Classification décimale de Dewey’, 23e édition [French translation of DDC23]
- the performance of Bach’s ‘Goldberg Variations’ by Angela Hewitt at St. Thomas Church (Leipzig Germany) in November 2020
- the performance of Bach’s ‘Goldberg Variations’ by Angela Hewitt in Christuskirche (Berlin) on 14-17 December 2015
- the musical score for Bach’s ‘Goldberg Variations’ (as published by Balthasar Schmid in 1741)
- Beethoven’s original score for Symphony No. 9 (as expressed by Beethoven’s original hand-written manuscript held by the Berlin State Library)
- the score for Beethoven’s Symphony No. 9 that was edited by Jonathan Del Mar and published by Bärenreiter in 1997
- the original cut of Hitchcock’s movie ‘Psycho’
- the censored version of Hitchcock’s movie ‘Psycho’ that was released in Britain (with stabbing sounds and visible nude shots removed)
- the first plaster version of ‘The Thinker’ sculpture made by Auguste Rodin around 1881
- large scale version of Auguste Rodin’s ‘The Thinker’ created at the Fonderie Alexis Rudier in 1904
</rdfs:comment>
  </owl:Class>
  <owl:Class rdf:about="F3_Manifestation">
    <rdfs:label xml:lang="en">F3 Manifestation</rdfs:label>
    <skos:notation>F3</skos:notation>
    <skos:prefLabel xml:lang="en">Manifestation</skos:prefLabel>
    <rdfs:subClassOf rdf:resource="http://www.cidoc-crm.org/cidoc-crm/E73_Information_Object"/>
    <rdfs:comment xml:lang="en">Scope note:
This class comprises products rendering one or more Expressions. A Manifestation is defined by both the overall content and the form of its presentation. The substance of F3 Manifestation is not only signs, but also the manner in which they are presented to be consumed by users, including the kind of media adopted.
An F3 Manifestation is the outcome of a publication process where one or more F2 Expressions are prepared for public dissemination, but it may also be a unique form created directly on some material carrier without the intent of being formally published.
An instance of F3 Manifestation typically incorporates one or more instances of F2 Expression representing a distinct logical content and all additional input by a publisher such as text layout and cover design. Additionally an F3 Manifestation can be identified by the physical features for the medium of distribution, if applicable. For example, publications in the form of hard-cover and paperback editions would be two distinct instances of F3 Manifestation, even though authorial and editorial content are otherwise identical in both publications.
In the case of industrial products such as printed books or music CDs, but also digital material, an instance of F3 Manifestation can be regarded as the prototype for all copies of it. In these cases, an instance of F3 Manifestation specifies all of the features or traits that instances of F5 Item display in order to be copies of a particular publication. In the case of industrial products, instances of F3 Manifestation are also instances of E99 Product Type, normally nowadays identified by characteristic identifiers such as ISBN numbers.

Examples:
- the publication ‘Murder on the Orient Express / Agatha Christie’, published by Collins Crime Club in 1934
- the publication of ‘Murder on the Orient Express / Agatha Christie’, published by HarperCollins in 2017
- the publication ‘Mord im Orientexpress : ein Hercule-Poirot-Roman / Agatha Christie’, published by Deutscher Bücherbund in 1975
- the publication ‘Murder on The Orient Express / Agatha Christie’, narrated by David Suchet, audio book (audio CD) published by HarperCollins in 2005
- the HTML-version of Homer’s ‘Odyssey’ with English text by S. H. Butcher and A. Lang, available online from the Gutenberg Project
- the publication ‘The Illustrated Odyssey’, published by Sidgwick &amp; Jackson Ltd in 1980, containing the translated text by E.V. Rieu, an introduction by Jacquetta Hawkes and photographs by Tim Mercer
- the publication ‘The Odyssey of Homer’ published by Harper &amp; Row in 1967, containing an introduction and the English translation of the Greek poem by Richmond Lattimore
- the CD publication ‘Bach Goldberg Variations’, published by Hyperion Records in 2016, containing a CD with Angela Hewitt’s performances of Bach’s ‘Goldberg Variations’ recorded in Christuskirche (Berlin) on 14-17 December 2015 and a booklet with an introduction to the music by Angela Hewitt in English, French and German
- the manuscript known as ‘The Book of Kells’
- the publication containing a text entitled ‘Pop Culture’ (authored by a person named ‘Richard Memeteau’), issued in 2014 by the publisher named ‘Zones’ and distributed in EPUB2 format by a distributor named ‘Editis’ and identified by ISBN ‘978-2-35522-085-2’
- the publication entitled ‘Alfred Hitchcock’s Psycho: 60th Anniversary Edition’, containing one Blu-ray disc with two cuts of the movie, released in 2020
</rdfs:comment>
  </owl:Class>
  <owl:Class rdf:about="F5_Item">
    <rdfs:label xml:lang="en">F5 Item</rdfs:label>
    <skos:notation>F5</skos:notation>
    <skos:prefLabel xml:lang="en">Item</skos:prefLabel>
    <rdfs:subClassOf rdf:resource="http://www.cidoc-crm.org/cidoc-crm/E24_Physical_Human-Made_Thing"/>
    <rdfs:comment xml:lang="en">Scope note:
This class comprises physical objects (printed books, scores, CDs, DVDs, CD-ROMS, etc.) that were produced by (P186i) an industrial process involving a given instance of F3 Manifestation. As a result, all the instances of F5 Item associated with a given instance of F3 Manifestation are expected to carry the content defined in that instance of F3 Manifestation, although some or even all of them may happen to carry a content that significantly differs from it, due to either an accident in the course of industrial production, or subsequent physical modification or degradation.
An instance of F5 Item that consists of a physical object or set of objects with clear physical boundaries is also an instance of E22 Human-Made Object. An instance of F5 Item that is stored on a part of a larger physical support (such as an electronic file among others on a disc) can also be considered to be an instance of E25 Human-Made Feature.
The notion of F5 Item is only relevant with regard to the production process, from a bibliographic point of view. The physical units managed by cultural heritage institutions in their holdings are a distinct notion: a unit of holdings certainly can be equal to an instance of F5 Item, but it also can be either “bigger” than one (e.g., when two instances of F5 Item are bound together (in the case of printed books)), or “smaller” than one (e.g., for incomplete holdings, such as when only one CD from a two-CD set is held). From an operational point of view, cultural heritage institutions typically do not manage instances of F5 Item, but physical holdings units, instances of E19 Physical Object, although for libraries in most cases this is not significant because each item corresponds with a single unit. When this is not the case, the linkage between items and the units relevant for collection management can be recorded through the P46 is composed of (forms part of) property between instances of F5 Item and instances of E19 Physical Object. If needed, an instance of E19 Physical Object can be typed as a unit through the P2 has type (is type of) property.

Examples:
- the copy of ‘Murder on the Orient Express / Agatha Christie’, HarperCollins 2017, that is held by the Deichman public library in Oslo, Norway, and which is identified by inventory number ‘9138513’
- John Smith’s copy of ‘Murder on the Orient Express / Agatha Christie’, HarperCollins 2017, with the owner’s ex libris stamped on the inside of the cover page
- the copy of the first edition of Bach’s ‘Goldberg Variations’ held by the National Library in France with corrections made by the composer, and additional music in the form of fourteen canons on the Goldberg ground
- the manuscript known as the ‘Book of Kells’ (owned by Trinity College in Dublin)
- the bronze statue of Auguste Rodin’s ‘The Thinker’, cast at the Fonderie Alexis Rudier in 1904 held at the Musée Rodin in Paris, France since 1922
- the ebook ‘Pop Culture’ by Richard Memeteau in EPUB2 format, received by the National Library of France through digital legal deposit on 1st February 2016 to which the legal deposit number DLN-20160201-6 has been assigned. In the catalogue, this item is identified with a unique number: LNUM20553886
- the copy of the electronic file named ‘cidoc_crm_version_7.1.3.pdf’ on my hard drive containing the text of official version 7.1.3 of the ‘Definition of the CIDOC Conceptual Reference Model’
</rdfs:comment>
  </owl:Class>
  <owl:Class rdf:about="F11_Corporate_Body">
    <rdfs:label xml:lang="en">F11 Corporate Body</rdfs:label>
    <skos:notation>F11</skos:notation>
    <skos:prefLabel xml:lang="en">Corporate Body</skos:prefLabel>
    <rdfs:subClassOf rdf:resource="http://iflastandards.info/ns/lrm/lrmoo/F55_Collective_Agent"/>
    <rdfs:comment xml:lang="en">Scope note:
This class comprises organisations and groups of two or more people and/or organisations acting as a unit.
To be considered an instance of F11 Corporate Body a gathering of people needs to bear a name and exhibit organisational characteristics sufficient to allow the body as a whole to participate in the creation, modification or production of an E73 Information Object. Groups such as conferences, congresses, expeditions, exhibitions, festivals, fairs, etc. are modelled as F11 Corporate Bodies when they are named and can take collective action, such as approving a report or publishing their proceedings.

Examples:
- The International Machaut Society
- The British Library
- The Jackson Five [pop band]
- Municipalité régionale de comté de Portneuf [regional municipality in Quebec]
- Symposium on Glaucoma
</rdfs:comment>
  </owl:Class>
  <owl:Class rdf:about="F12_Nomen">
    <rdfs:label xml:lang="en">F12 Nomen</rdfs:label>
    <skos:notation>F12</skos:notation>
    <skos:prefLabel xml:lang="en">Nomen</skos:prefLabel>
    <rdfs:subClassOf rdf:resource="http://www.cidoc-crm.org/cidoc-crm/E89_Propositional_Object"/>
    <rdfs:comment xml:lang="en">Scope note:
This class comprises associations between an instance of any class, and signs or arrangements of signs that are used to refer to and identify that instance.
Signs include alphanumeric characters, ideograms, notations such as chemical structure symbols, sound symbols, etc. The scripts or type sets for the symbols used to compose an instance of F12 Nomen have to be sufficiently specified. Spelling variants are regarded as different nomens, whereas the use of different fonts (visual representation variants) or different digital encodings do not change the identity.
An arbitrary combination of signs or symbols cannot be regarded as an appellation or designation until it is associated with something in some context. In that sense, the F12 Nomen class can be understood as the reification of a relationship between an instance of E1 CRM Entity and an instance of E41 Appellation. Two instances of F12 Nomen can happen to be associated with equivalent strings and yet remain distinct, as long as they refer to distinct instances of E1 CRM Entity. Furthermore, two instances of F12 Nomen referring to the same instance of E1 CRM Entity may be associated with equivalent strings, and remain distinct as long as they are associated with distinct properties of the F12 Nomen class (for example, having the same spelling in different languages, or being defined in different controlled vocabularies).
An instance of F12 Nomen associates a combination of signs with an instance of E1 CRM Entity on the basis of a cultural or linguistic convention: by associating a string with anything, the instance of F12 Nomen establishes a meaning that is not inherent in the instance of E62 String that is associated with it. Depending on context of use, nomens associated with equivalent strings can be associated with instances of different things in the real world even within the same language (polysemy and homonymy). Conversely, the same thing can be referred to through any number of nomens (synonymy). In the controlled environment of a bibliographic information system, though, homonymy is avoided.
Instances of F12 Nomen are assigned and associated with instances of E1 CRM Entity either formally (such as by bibliographic agencies) or informally through common usage. When they are assigned formally, the construction of the instances of E62 String that represent them may follow predetermined rules.

Examples:
- ‘杜甫’ as the name for a Chinese poet of the 8(th) century, rendered in simplified Chinese characters
- ‘Du Fu’ as the name for a Chinese poet of the 8(th) century, rendered in Pinyin romanised form
- ‘Tu Fu’ as the name for a Chinese poet of the 8(th) century, rendered in another romanised form
- ‘Thơ Ðô Phủ’ as the name for a Chinese poet of the 8(th) century, rendered in a Vietnamese form
- ‘جامعة صفاقس’ as the name for Sfax University (Tunisia), rendered in Arabic in Arabic script
- ‘Ğāmi‘at̀̀ Ṣafāqis’ as the name for Sfax University (Tunisia), rendered in transliterated Arabic
- ‘Université de Sfax’ as the name for Sfax University (Tunisia), rendered in French
- ‘3-[(2S)-1-methylpyrrolidin-2-yl]pyridine’ as the term for nicotine, rendered in the IUPAC nomenclature of organic chemistry
- ‘Murders in the rue Morgue’ as the title of the textual work by Edgar Allan Poe, in English
- ‘Poe, Edgar Allan, 1809-1849. Murders in the rue Morgue’ as the name of the textual work, formulated as a controlled author/title access point appropriate for an English language catalogue
- ‘modelling’ as the term for the activity, in English using British spelling
- ‘modeling’ as the term for the activity, in English using American spelling
- ‘Maxwell equations’ as the term for these equations, formulated as the preferred subject access point from LCSH, http://lccn.loc.gov/sh85082387, as of 27 March 2012 [date of last update]
- ‘Equations, Maxwell’ as the term for these equations, formulated as a variant subject access point, from the same source
- ‘Gontcharova, Nathalie (1881-1962)’ as the name of the Russian artist, formulated as an preferred access point from the authority file of the National Library of France, http://catalogue.bnf.fr/ark:/12148/cb119547494/PUBLIC, as of 11 March 2015 [date of last update]
- ‘Gončarova, Natalʹâ Sergeevna (1881-1962)’ as the name of the Russian artist, formulated as a variant access point for a personal name, transliterated using ISO 9:1995 ‘Information and documentation — Transliteration of Cyrillic characters into Latin characters — Slavic and non-Slavic languages’, also from the authority file of the National Library of France
- ‘Гончарова, Наталья Сергеевна (1881-1962)’ as the name of the Russian artist, formulated as a variant access point in Cyrillic script, also from the authority file of the National Library of France
- ‘595.7’ as a classification number for insects (the taxonomic class Insecta), in the 23rd edition of the Dewey Decimal Classification
- ‘Insecta’ as a term for insects (the taxonomic class Insecta), used as the caption for the class ‘595.7’ in the English language 23rd edition of the Dewey Decimal Classification
- ‘spa’ as a code to designate the language Spanish, drawn from set 2 (3-letter language identifiers) of ‘ISO 639 – Code for individual languages and language groups’ (ISO 639:2023)
</rdfs:comment>
  </owl:Class>
  <owl:Class rdf:about="F18_Serial_Work">
    <rdfs:label xml:lang="en">F18 Serial Work</rdfs:label>
    <skos:notation>F18</skos:notation>
    <skos:prefLabel xml:lang="en">Serial Work</skos:prefLabel>
    <rdfs:subClassOf rdf:resource="http://iflastandards.info/ns/lrm/lrmoo/F1_Work"/>
    <rdfs:comment xml:lang="en">Scope note:
This class comprises works that are, or have been, planned to result in sequences of Expressions or Manifestations with common features. Whereas a work can acquire new members during the time it evolves, Expressions and Manifestations are identified with a certain state achieved at a particular point in time. Therefore there is in general no single Expression or Manifestation representing a complete serial work, unless the serial work has ended.
Serial Works may or may not have a plan for an overall expression.
The retrospective reprinting of all issues of a Serial Work at once, in the form of a monograph, is regarded to be another member of the F1 Work, which contains the Serial Work and the Work realised in the monograph. This does not make the monograph part of the Serial Work.

Examples:
- the periodical entitled ‘The UNESCO Courier’, ISSN ‘0041-5278’
- the periodical entitled ‘Courrier de l’UNESCO’, ISSN ‘0304-3118’ [French edition of the periodical titled ‘The UNESCO Courier’, ISSN ‘0041-5278’]
- the series entitled ‘L’évolution de l’humanité’, ISSN ‘0755-1843’ [a monograph series comprising volumes that were published from 1920 on, and some of which were reprinted, with different physical features and rearranged in a different order, from 1968 on, in a distinct series also entitled ‘L’évolution de l’humanité’, ISSN ‘0755-1770’]
</rdfs:comment>
  </owl:Class>
  <owl:Class rdf:about="F27_Work_Creation">
    <rdfs:label xml:lang="en">F27 Work Creation</rdfs:label>
    <skos:notation>F27</skos:notation>
    <skos:prefLabel xml:lang="en">Work Creation</skos:prefLabel>
    <rdfs:subClassOf rdf:resource="http://www.cidoc-crm.org/cidoc-crm/E65_Creation"/>
    <rdfs:comment xml:lang="en">Scope note:
This class comprises activities by which instances of F1 Work come into existence. An instance of F27 Work Creation can serve to document the period a work was coming into existence and the circumstances of it, when these are known.
An instance of F27 Work Creation marks the initial creation of an instance of F1 Work through expressions or other externalisations that are sufficiently elaborated so that the characteristic conceptual identity of the work could be recognized as existing.
In many cases this will coincide with the first known complete externalisation of an expression of the work. In other cases, the initial creation of an instance of F1 Work may be inferred from multiple, or later, expressions or other forms of evidence. For instance, commissioning of a work may explicitly be agreed on after the presentation of an already complete and detailed elaboration of the work that was not made public. Performances may be prior to written expressions, as in the case of Shakespeare’s works.
The work, as an intellectual construction, may evolve from its initial creation onwards, until the last known expression of it.
An instance of E39 Actor with which a work is associated through the chain of properties F1 Work. R16i was created by: F27 Work Creation. P14 carried out by (performed): E39 Actor corresponds to the notion of the “creator” of the work.
In the situation where an expression of one instance of F1 Work serves as source material for the creation of the first expression of a new instance of F1 Work, the direct relationship between the works is indicated using the property R2 is derivative of (has derivative) between the two instances of F1 Work. The link to the specific source expression is indicated with the property P16 used specific object (was used for) using the path: F1 Work(1). R3 is realised in: F2 Expression(1). P16i was used for: F27 Work Creation. R16 created: F1 Work(2).

Examples:
- Agatha Christie creating ‘Murder on the Orient Express’
- Mary Shelley creating ‘Frankenstein, or, The Modern Prometheus’
- Dante creating the poem ‘Divina Commedia’
- William Shakespeare creating ‘The Tragedy of Hamlet, Prince of Denmark’
- René Goscinny and Albert Uderzo (collaboratively) creating ‘Astérix le Gaulois’
- Ludwig van Beethoven composing his Symphony No. 9
- Johann Sebastian Bach composing the ‘Goldberg Variations’
- the making of ‘Jules et Jim’, directed by François Truffault
- the making of ‘Psycho’, directed by Alfred Hitchcock
- Auguste Rodin creating ‘Le Penseur’ (‘The Thinker’)
- Picasso creating ‘Guernica’
- Pascal Bonnefois and Marie-Louise Ollier creating ‘Yvain ou Le chevalier au lion : concordance lemmatisée’ [a concordance for the novel ‘Le chevalier au lion’ by Chrétien de Troyes, based on the 1960 edition by Mario Roques]
</rdfs:comment>
  </owl:Class>
  <owl:Class rdf:about="F28_Expression_Creation">
    <rdfs:label xml:lang="en">F28 Expression Creation</rdfs:label>
    <skos:notation>F28</skos:notation>
    <skos:prefLabel xml:lang="en">Expression Creation</skos:prefLabel>
    <rdfs:subClassOf rdf:resource="http://www.cidoc-crm.org/cidoc-crm/E12_Production"/>
    <rdfs:subClassOf rdf:resource="http://www.cidoc-crm.org/cidoc-crm/E65_Creation"/>
    <rdfs:comment xml:lang="en">Scope note:
This class comprises activities that result in instances of F2 Expression coming into existence. An instance of F2 Expression is considered to be created when it is captured on a carrier other than the creator’s brain.
Although F2 Expression is an abstract entity, a conceptual object, the creation of an expression inevitably also affects the physical world: when you scribble the first draft of a poem on a sheet of paper, you produce an instance of F3 Manifestation and an instance of F5 Item. F28 Expression Creation is a subclass of E12 Production because the recording of the expression causes a physical modification of the E18 Physical Thing that serves as the carrier. The creation of an instance of F2 Expression coincides with the creation of the first instance of F3 Manifestation that R4 embodies (is embodied in) this instance of F2 Expression.
The P2 has type (is type of) property can be used to specify the type of the instance of F28 Expression Creation (i.e., activities such as translating, revising, or arranging music are types of creation process). The type of the process is distinct from the type of result even though the typology frequently used for instances of the resulting F2 Expressions may imply the category of the instance of the F28 Expression Creation.
An instance of F28 Expression Creation may use as source material one or more specific instances of F2 Expression. When the source expression is documented this is also expressed by the property R76 is derivative of (has derivative).

Examples:
- Agatha Christie writing the original manuscript for ‘Murder on the Orient Express’
- Elisabeth van Bebber creating the German translation of ‘Murder on the Orient Express’
- Angela Hewitt performing the ‘Goldberg Variations’ at St. Thomas Church (Leipzig Germany) in November 2020
- Angela Hewitt performing the ‘Goldberg Variations’ in Christuskirche (Berlin) on 14-17 December 2015 (for a CD production)
- Beethoven scripting the original score for the 9(th) symphony
- Jonathan Del Mar editing and creating the score for Beethoven’s 9(th) symphony (as published by Bärenreiter in 1997)
- the making of the original cut of Hitchcock’s movie ‘Psycho’
- the making of the censored version of Hitchcock’s movie ‘Psycho’ that was released in Britain
- Auguste Rodin making the first plaster version of ‘The Thinker’ sculpture
- the making of the large-scale version of ‘The Thinker’ by the ‘Fonderie Alexis Rudier in 1904
</rdfs:comment>
  </owl:Class>
  <owl:Class rdf:about="F30_Manifestation_Creation">
    <rdfs:label xml:lang="en">F30 Manifestation Creation</rdfs:label>
    <skos:notation>F30</skos:notation>
    <skos:prefLabel xml:lang="en">Manifestation Creation</skos:prefLabel>
    <rdfs:subClassOf rdf:resource="http://www.cidoc-crm.org/cidoc-crm/E12_Production"/>
    <rdfs:subClassOf rdf:resource="http://www.cidoc-crm.org/cidoc-crm/E65_Creation"/>
    <rdfs:comment xml:lang="en">Scope note:
This class comprises the activities of selecting, arranging and presenting one or more instances of F2 Expression on a carrier or other persistent presentation means with the purpose of communicating it to some public. It includes the specification of the presentation as to sensory impression (such as visual appearance or audio rendition).

Examples:
- the process of creating the publication ‘Murder on the Orient Express / Agatha Christie’, published by HarperCollins in 2017, including deciding the format, typesetting the text, designing the cover and other features of the publication
- the process of making the HTML-version of the English text of Homer’s ‘Odyssey’ (translated by S. H. Butcher and A. Lang), which is available online from the Gutenberg Project
- the process of making the engraved copper plates for the first edition of Bach’s ‘Goldberg Variations’ by Balthasar Schmid
- the process of making the CD publication ‘Bach Goldberg Variations’, published by Hyperion Records in 2016, including the process of recording the performance, editing, and typesetting the booklet, and design of the overall publication
</rdfs:comment>
  </owl:Class>
  <owl:Class rdf:about="F31_Performance">
    <rdfs:label xml:lang="en">F31 Performance</rdfs:label>
    <skos:notation>F31</skos:notation>
    <skos:prefLabel xml:lang="en">Performance</skos:prefLabel>
    <rdfs:subClassOf rdf:resource="http://www.cidoc-crm.org/cidoc-crm/E7_Activity"/>
    <rdfs:comment xml:lang="en">Scope note:
This class comprises activities where an instance of F1 Work is presented or communicated directly or indirectly to an audience, such as a theatrical play, a musical work or a choreographic work.
Performances can be identified at various levels of granularity, but an instance of F31 Performance is always associated with a single identified instance of F1 Work. An instance of F31 Performance may consist of other instances of F31 Performance as parts, such as a piano concerto that has multiple movements. In addition, a complete run of equivalent performances of the same work can also be seen as an instance of F31 Performance, with the individual performances as parts.
Activities that include performing multiple individual works, e.g., that are put together as a program for a show or concert, but where the activity as a whole is not associated with an instance of F1 Work, should be represented as instances of E7 Activity consisting of individual instances of F31 Performances as parts (the property P9 consists of (forms part of) expresses the relationship).
Instances of F31 Performance may be created according to specific staging directions, be based on specific known instances of F2 Expression (such as translations), or be influenced by or include elements that relate to different works other than the single work the performance is dominated by. This can be documented using the properties P16 used specific object (was used for) or P15 was influenced by (influenced).

Examples:
- the performance of a Yiddish translation of the textual work entitled ‘King Lear’, as directed by Sergei Radlov, in Moscow, at the Moscow State Jewish Theatre, on February 10, 1935
- the performance of the ballet entitled ‘Rite of spring’, as choreographed by Pina Bausch, in Avignon, at the Popes’ Palace, on July 7, 1995
- the performance of the operatic work entitled ‘Dido and Aeneas’, as directed by Edward Gordon Craig and conducted by Martin Shaw, in London, Hampstead Conservatoire, on May 17, 18, and 19, 1900
- the performance of Verdi’s ‘La Traviata’ at the Salzburg Festival in 2005, that was staged by Willy Decker, directed by Brian Large and featuring Anna Netrebko and Rolando Villazón
- the performance of Michel Fokine’s choreography and libretto (choreographic work) for Stravinsky’s ‘The Firebird’ by the Mariinsky Orchestra and Ballet at the Mariinsky Theatre in Saint Petersburg, June 2008
- the performance of Daniel Humair and Damien Varaillon’s improvisation ‘Hommage à John Coltrane’ in the Bal Blomet (Paris), on 18 January 2018
</rdfs:comment>
  </owl:Class>
  <owl:Class rdf:about="F32_Item_Production_Event">
    <rdfs:label xml:lang="en">F32 Item Production Event</rdfs:label>
    <skos:notation>F32</skos:notation>
    <skos:prefLabel xml:lang="en">Item Production Event</skos:prefLabel>
    <rdfs:subClassOf rdf:resource="http://www.cidoc-crm.org/cidoc-crm/E12_Production"/>
    <rdfs:comment xml:lang="en">Scope note:
This class comprises activities that result in one or more instances of F5 Item coming into existence. The production of a series of physical objects (printed books, scores, CDs, DVDs, CD-ROMs, etc.), producing a unique item (writing a manuscript on parchment, painting a watercolour, etc.), and the creation of a new copy of a file on an electronic carrier are all regarded as instances of F32 Item Production Event.
For mass-produced items, the production process (no matter whether it is a book, a sound recording, a DVD, a cartographic resource, etc.) strives to produce items all as similar as possible to a prototype that displays all the features that all the copies of the publication should also display, which is reflected in the property R27 materialized: F3 Manifestation.

Examples:
- the printing and binding of copies of the paperback edition of the HarperCollins 2017 publication ‘Murder on the Orient Express / Agatha Christie’, by CPI Ltd (UK)
- the printing of copies of the score of Bach’s ‘Goldberg Variations’ by Balthasar Schmid in 1741
- the casting of Auguste Rodin’s ‘The Thinker’ at the Fonderie Alexis Rudier in 1904
- the production of the items of the CD publication ‘Bach Goldberg Variations’, published by Hyperion Records in 2016, including the pressing of the CDs, the printing of the booklet and cover, assembling the parts, etc.
</rdfs:comment>
  </owl:Class>
  <owl:Class rdf:about="F33_Reproduction_Event">
    <rdfs:label xml:lang="en">F33 Reproduction Event</rdfs:label>
    <skos:notation>F33</skos:notation>
    <skos:prefLabel xml:lang="en">Reproduction Event</skos:prefLabel>
    <rdfs:subClassOf rdf:resource="http://iflastandards.info/ns/lrm/lrmoo/F30_Manifestation_Creation"/>
    <rdfs:subClassOf rdf:resource="http://www.cidoc-crm.org/cidoc-crm/E12_Production"/>
    <rdfs:comment xml:lang="en">Scope note:
This class comprises activities that consist in producing items of a new instance of F3 Manifestation that preserve both the content and layout found on items of a pre-existing instance of F3 Manifestation. The individual instance or instances of F5 Item that was or were used as a source for this process may be precisely identified or not. Such activities result in products known as facsimiles, reproductions, reprints, reissues, or new releases.

Examples:
- the 2014 publication of Daniel Wilson’s ‘Caliban: the missing link’ by Cambridge University Press [a facsimile edition of the 1873 publication by Macmillan]
- the 2015 publication of Harry Partch’s ‘Two studies on ancient Greek scales’ by Schott [which reproduces Harry Partch’s holograph manuscript]
- the 2007 publication of Hubert Reeve’s ‘Malicorne: réflexions d’un observateur de la nature’ published by Éditions du Seuil as number 179 in the series ‘Points. Science’ (ISBN ‘978-2-02-096760-0’) [a reprint edition of the 1990 publication by Éditions du Seuil in the series ‘Science ouverte’ (ISBN ‘2-02-012644-3’)]
</rdfs:comment>
  </owl:Class>
  <owl:Class rdf:about="F36_Script_Conversion">
    <rdfs:label xml:lang="en">F36 Script Conversion</rdfs:label>
    <skos:notation>F36</skos:notation>
    <skos:prefLabel xml:lang="en">Script Conversion</skos:prefLabel>
    <rdfs:subClassOf rdf:resource="http://www.cidoc-crm.org/cidoc-crm/E29_Design_or_Procedure"/>
    <rdfs:comment xml:lang="en">Scope note:
This class comprises rule sets for converting signs or arrangements of signs from one script or type set to another.

Examples:
- the rules for the transliteration of the Cyrillic script into Latin script codified in ISO 9:1995 ‘Information and documentation — Transliteration of Cyrillic characters into Latin characters — Slavic and non-Slavic languages’ (ISO 9:1995)
</rdfs:comment>
  </owl:Class>
  <owl:Class rdf:about="F39_Family">
    <rdfs:label xml:lang="en">F39 Family</rdfs:label>
    <skos:notation>F39</skos:notation>
    <skos:prefLabel xml:lang="en">Family</skos:prefLabel>
    <rdfs:subClassOf rdf:resource="http://iflastandards.info/ns/lrm/lrmoo/F55_Collective_Agent"/>
    <rdfs:comment xml:lang="en">Scope note:
This class comprises groups of two or more persons presented as a family and justified by relationships of birth, marriage, adoption, civil union, or similar social or legal status and an assumed common tradition, including examples such as royal families, dynasties, houses of nobility, etc.

Examples:
- House of Tudor
- the brothers Grimm
</rdfs:comment>
  </owl:Class>
  <owl:Class rdf:about="F55_Collective_Agent">
    <rdfs:label xml:lang="en">F55 Collective Agent</rdfs:label>
    <skos:notation>F55</skos:notation>
    <skos:prefLabel xml:lang="en">Collective Agent</skos:prefLabel>
    <rdfs:subClassOf rdf:resource="http://www.cidoc-crm.org/cidoc-crm/E74_Group"/>
    <rdfs:comment xml:lang="en">Scope note:
This class comprises recognizable groups or organizations of persons that have the potential of acting as a unit to produce some intentional result of bibliographic interest for which they can be collectively considered responsible.
A group of people becomes an instance of F55 Collective Agent when it identifies itself by a name that identifies it within an appropriate context and exhibits sufficient organizational characteristics to permit it to perform actions that reflect agency. Groups that are constituted as meetings, conferences, congresses, expeditions, festivals, fairs, etc. are examples of F55 Collective Agent as long as they self-identify by a specific name, rather than being referred to by a generic description of the gathering, and can act as a unit (such as by publishing their proceedings, or approving a report). These collective actions may be performed by representatives selected by the whole, rather than by all individual members acting together.
Collective Agents may be members of other Collective Agents, although directly or indirectly all Collective Agents are composed of persons. The membership of many types of Collective Agents will continue to evolve over time. A Collective Agent may continue to exist even if it has no members for a time (for example, a committee whose members all resign prior to the expiration of their terms but then a new complement of members is appointed).
Instances of F55 Collective Agent include instances of its subclass F11 Corporate Body: commercial or corporate entities and other legally registered bodies, as well as organizations and associations, musical, artistic or performing groups, governments, and any of their sub-units.
Married couples and other concepts of family (instances of F39 Family) are instances of a subclass of F55 Collective Agent.
In the wider sense, this class also comprises holders of official positions viewed collectively, independent of the current holder of the office, such as the president of a country. In such cases, it is possible that the instance of F55 Collective Agent has only ever had a single member.
A group of persons known by/using a joint pseudonym (i.e., a name that seems indicative of an individual but that is actually adopted as a persona by two or more people acting together) is a case of F55 Collective Agent.

Examples:
- International Federation of Library Associations and Institutions (F11)
- 81st World Library and Information Conference (F11)
- Bibliothèque nationale de France (F11)
- Exxon-Mobil (F11)
- The Beatles (F11)
- the brothers Grimm (F39)
- the President of the Swiss Confederation
- Nicolas Bourbaki [collective pseudonym of a group of 20(th) century French mathematicians also known as the ‘Association des collaborateurs de Nicolas Bourbaki’]
- Ellery Queen [joint pseudonym for detective fiction of cousins Frederic Dannay and Manfred Bennington Less who also wrote separately]
</rdfs:comment>
  </owl:Class>
  <owl:ObjectProperty rdf:about="R1_is_logical_successor_of">
    <rdfs:label xml:lang="en">R1 is logical successor of</rdfs:label>
    <skos:notation>R1</skos:notation>
    <skos:prefLabel xml:lang="en">is logical successor of</skos:prefLabel>
    <rdfs:domain rdf:resource="http://iflastandards.info/ns/lrm/lrmoo/F1_Work"/>
    <rdfs:range rdf:resource="http://iflastandards.info/ns/lrm/lrmoo/F1_Work"/>
    <owl:inverseOf rdf:resource="http://iflastandards.info/ns/lrm/lrmoo/R1i_has_successor"/>
    <rdfs:subPropertyOf rdf:resource="http://www.cidoc-crm.org/cidoc-crm/P130_shows_features_of"/>
    <rdfs:comment xml:lang="en">Quantification: many to many (0,n:0,n)

Scope note:
This property associates an instance of F1 Work which logically continues the content of another instance of F1 Work with the latter. This property is not transitive. It is asymmetric and irreflexive.

Examples:
- Ursula K. Le Guin’s novel ‘The Tombs of Atuan’ (F1) is logical successor of Ursula K. Le Guin’s novel ‘A Wizard of Earthsea’ (F1).
- Miguel de Cervantes’ ‘Segunda Parte del Ingenioso Cavallero Don Quixote de la Mancha’ (F1) is logical successor of Miguel de Cervantes’ ‘El ingenioso hidalgo Don Quixote de la Mancha’ (F1).
- The TV series ‘Breaking Bad’ (F1) is logical successor of the TV series ‘Better Call Saul’ (F1).
- The first ‘Star Wars’ trilogy, 1977-1983 (F1) is logical successor of the second ‘Star Wars’ trilogy, 1999-2005 (F1). [Note that the logical order does not follow, in either of the two last examples, the chronological order of creation]
</rdfs:comment>
  </owl:ObjectProperty>
  <owl:ObjectProperty rdf:about="R1i_has_successor">
    <rdfs:label xml:lang="en">R1i has successor</rdfs:label>
    <skos:notation>R1i</skos:notation>
    <skos:prefLabel xml:lang="en">has successor</skos:prefLabel>
    <rdfs:domain rdf:resource="http://iflastandards.info/ns/lrm/lrmoo/F1_Work"/>
    <rdfs:range rdf:resource="http://iflastandards.info/ns/lrm/lrmoo/F1_Work"/>
    <owl:inverseOf rdf:resource="http://iflastandards.info/ns/lrm/lrmoo/R1_is_logical_successor_of"/>
    <rdfs:subPropertyOf rdf:resource="http://www.cidoc-crm.org/cidoc-crm/P130i_features_are_also_found_on"/>
    <rdfs:comment xml:lang="en">Quantification of the inverse property: many to many (0,n:0,n)

Scope note of the inverse property:
This property associates an instance of F1 Work which logically continues the content of another instance of F1 Work with the latter. This property is not transitive. It is asymmetric and irreflexive.

Examples of the inverse property:
- Ursula K. Le Guin’s novel ‘The Tombs of Atuan’ (F1) is logical successor of Ursula K. Le Guin’s novel ‘A Wizard of Earthsea’ (F1).
- Miguel de Cervantes’ ‘Segunda Parte del Ingenioso Cavallero Don Quixote de la Mancha’ (F1) is logical successor of Miguel de Cervantes’ ‘El ingenioso hidalgo Don Quixote de la Mancha’ (F1).
- The TV series ‘Breaking Bad’ (F1) is logical successor of the TV series ‘Better Call Saul’ (F1).
- The first ‘Star Wars’ trilogy, 1977-1983 (F1) is logical successor of the second ‘Star Wars’ trilogy, 1999-2005 (F1). [Note that the logical order does not follow, in either of the two last examples, the chronological order of creation]
</rdfs:comment>
  </owl:ObjectProperty>
  <owl:ObjectProperty rdf:about="R2_is_derivative_of">
    <rdfs:label xml:lang="en">R2 is derivative of</rdfs:label>
    <skos:notation>R2</skos:notation>
    <skos:prefLabel xml:lang="en">is derivative of</skos:prefLabel>
    <rdfs:domain rdf:resource="http://iflastandards.info/ns/lrm/lrmoo/F1_Work"/>
    <rdfs:range rdf:resource="http://iflastandards.info/ns/lrm/lrmoo/F1_Work"/>
    <owl:inverseOf rdf:resource="http://iflastandards.info/ns/lrm/lrmoo/R2i_has_derivative"/>
    <rdfs:subPropertyOf rdf:resource="http://iflastandards.info/ns/lrm/lrmoo/R68_is_inspired_by"/>
    <rdfs:comment xml:lang="en">Quantification: many to many (0,n:0,n)

Scope note:
This property associates an instance of F1 Work which modifies the content of another instance of F1 Work with the latter. This property is transitive, asymmetric and irreflexive.
The inverse of this property is equivalent to the developed path: F1 Work(1). R3 is realised in: F2 Expression(1). P16i was used for: F28 Expression Creation. R17 created: F2 Expression(2). R3i realises: F1 Work(2). That is, F1 Work(1). R2i has derivative: F1 Work (2), without needing to specify the specific expressions involved in the derivation.

Examples:
- The movie ‘Murder on the Orient Express’ directed by Kenneth Branagh (F1) is derivative of the novel ‘Murder on the Orient Express’ by Agatha Christie (F1) with has type Movie adaptation (E55).
- The movie ‘A Clockwork Orange’ directed by Stanley Kubrick (F1) is derivative of the novel ‘A Clockwork Orange’ by Anthony Burgess (F1) with has type Movie adaptation (E55).
- Seth Grahame-Smith’s novel ‘Pride and prejudice and zombies’(F1) is derivative of Jane Austen’s novel ‘Pride and prejudice’ (F1) with has type Parody (E55).

Properties:
- R2.1 has type: 
  Scope note:
    This property allows for specifying the kind of derivation, such as adaptation, summarisation, etc.
</rdfs:comment>
  </owl:ObjectProperty>
  <owl:ObjectProperty rdf:about="R2i_has_derivative">
    <rdfs:label xml:lang="en">R2i has derivative</rdfs:label>
    <skos:notation>R2i</skos:notation>
    <skos:prefLabel xml:lang="en">has derivative</skos:prefLabel>
    <rdfs:domain rdf:resource="http://iflastandards.info/ns/lrm/lrmoo/F1_Work"/>
    <rdfs:range rdf:resource="http://iflastandards.info/ns/lrm/lrmoo/F1_Work"/>
    <owl:inverseOf rdf:resource="http://iflastandards.info/ns/lrm/lrmoo/R2_is_derivative_of"/>
    <rdfs:subPropertyOf rdf:resource="http://iflastandards.info/ns/lrm/lrmoo/R68i_is_inspiration_for"/>
    <rdfs:comment xml:lang="en">Quantification of the inverse property: many to many (0,n:0,n)

Scope note of the inverse property:
This property associates an instance of F1 Work which modifies the content of another instance of F1 Work with the latter. This property is transitive, asymmetric and irreflexive.
The inverse of this property is equivalent to the developed path: F1 Work(1). R3 is realised in: F2 Expression(1). P16i was used for: F28 Expression Creation. R17 created: F2 Expression(2). R3i realises: F1 Work(2). That is, F1 Work(1). R2i has derivative: F1 Work (2), without needing to specify the specific expressions involved in the derivation.

Examples of the inverse property:
- The movie ‘Murder on the Orient Express’ directed by Kenneth Branagh (F1) is derivative of the novel ‘Murder on the Orient Express’ by Agatha Christie (F1) with has type Movie adaptation (E55).
- The movie ‘A Clockwork Orange’ directed by Stanley Kubrick (F1) is derivative of the novel ‘A Clockwork Orange’ by Anthony Burgess (F1) with has type Movie adaptation (E55).
- Seth Grahame-Smith’s novel ‘Pride and prejudice and zombies’(F1) is derivative of Jane Austen’s novel ‘Pride and prejudice’ (F1) with has type Parody (E55).
</rdfs:comment>
  </owl:ObjectProperty>
  <owl:ObjectProperty rdf:about="R3_is_realised_in">
    <rdfs:label xml:lang="en">R3 is realised in</rdfs:label>
    <skos:notation>R3</skos:notation>
    <skos:prefLabel xml:lang="en">is realised in</skos:prefLabel>
    <rdfs:domain rdf:resource="http://iflastandards.info/ns/lrm/lrmoo/F1_Work"/>
    <rdfs:range rdf:resource="http://iflastandards.info/ns/lrm/lrmoo/F2_Expression"/>
    <owl:inverseOf rdf:resource="http://iflastandards.info/ns/lrm/lrmoo/R3i_realises"/>
    <rdfs:subPropertyOf rdf:resource="http://www.cidoc-crm.org/cidoc-crm/P130_shows_features_of"/>
    <rdfs:comment xml:lang="en">Quantification: one to many, necessary, dependent (1,n:1,1)

Scope note:
This property associates an instance of F2 Expression with an instance of F1 Work.
This property expresses the association that exists between an expression and the work that this expression conveys. Our factual knowledge of how a given work is historically realised into expressions is often limited. Therefore, this property makes it possible to express the association between an instance of F2 Expression and the instance of F1 Work it conveys without identifying the particular instances of F2 Expression that were part of a chain of derivation from the source.

Examples:
- Agatha Christie’s work entitled ‘Murder on the Orient Express’ (F1) is realised in the original text written by Agatha Christie for the novel (F2).
- Agatha Christie’s work entitled ‘Murder on the Orient Express’ (F1) is realised in the German translation created by Elisabeth van Bebber (F2).
- Agatha Christie’s work entitled ‘Murder on the Orient Express’ (F1) is realised in the narration of the English text by David Suchet (F2).
- Dante’s work entitled ‘Inferno’ (F1) is realised in the Italian text of Dante’s ‘Inferno’ as found in the authoritative critical edition ‘La Commedia secondo l’antica issolu’ a cura di Giorgio Petrocchi, Milano: Mondadori, 1966-67 (= ‘Le Opere di Dante Alighieri’, Edizione Nazionale a cura della Società Dantesca Italiana, VII, 1-4) (F2).
- Johann Sebastian Bach’s ‘Goldberg Variations’ (F1) is realised in the score of the ‘Goldberg Variations’ (as published by Balthasar Schmid in 1741) (F2).
- Auguste Rodin’s work ‘The Thinker’ (F1) is realised in the first plaster version of ‘The thinker’ (F2) that Auguste Rodin made around 1881.
- Auguste Rodin’s work ‘The Thinker’ (F1) is realised in the large-scale version of ‘The thinker’ (F2) created at the Fonderie Alexis Rudier in 1904.
</rdfs:comment>
  </owl:ObjectProperty>
  <owl:ObjectProperty rdf:about="R3i_realises">
    <rdfs:label xml:lang="en">R3i realises</rdfs:label>
    <skos:notation>R3i</skos:notation>
    <skos:prefLabel xml:lang="en">realises</skos:prefLabel>
    <rdfs:domain rdf:resource="http://iflastandards.info/ns/lrm/lrmoo/F2_Expression"/>
    <rdfs:range rdf:resource="http://iflastandards.info/ns/lrm/lrmoo/F1_Work"/>
    <owl:inverseOf rdf:resource="http://iflastandards.info/ns/lrm/lrmoo/R3_is_realised_in"/>
    <rdfs:subPropertyOf rdf:resource="http://www.cidoc-crm.org/cidoc-crm/P130i_features_are_also_found_on"/>
    <rdfs:comment xml:lang="en">Quantification of the inverse property: one to many, necessary, dependent (1,n:1,1)

Scope note of the inverse property:
This property associates an instance of F2 Expression with an instance of F1 Work.
This property expresses the association that exists between an expression and the work that this expression conveys. Our factual knowledge of how a given work is historically realised into expressions is often limited. Therefore, this property makes it possible to express the association between an instance of F2 Expression and the instance of F1 Work it conveys without identifying the particular instances of F2 Expression that were part of a chain of derivation from the source.

Examples of the inverse property:
- Agatha Christie’s work entitled ‘Murder on the Orient Express’ (F1) is realised in the original text written by Agatha Christie for the novel (F2).
- Agatha Christie’s work entitled ‘Murder on the Orient Express’ (F1) is realised in the German translation created by Elisabeth van Bebber (F2).
- Agatha Christie’s work entitled ‘Murder on the Orient Express’ (F1) is realised in the narration of the English text by David Suchet (F2).
- Dante’s work entitled ‘Inferno’ (F1) is realised in the Italian text of Dante’s ‘Inferno’ as found in the authoritative critical edition ‘La Commedia secondo l’antica issolu’ a cura di Giorgio Petrocchi, Milano: Mondadori, 1966-67 (= ‘Le Opere di Dante Alighieri’, Edizione Nazionale a cura della Società Dantesca Italiana, VII, 1-4) (F2).
- Johann Sebastian Bach’s ‘Goldberg Variations’ (F1) is realised in the score of the ‘Goldberg Variations’ (as published by Balthasar Schmid in 1741) (F2).
- Auguste Rodin’s work ‘The Thinker’ (F1) is realised in the first plaster version of ‘The thinker’ (F2) that Auguste Rodin made around 1881.
- Auguste Rodin’s work ‘The Thinker’ (F1) is realised in the large-scale version of ‘The thinker’ (F2) created at the Fonderie Alexis Rudier in 1904.
</rdfs:comment>
  </owl:ObjectProperty>
  <owl:ObjectProperty rdf:about="R4_embodies">
    <rdfs:label xml:lang="en">R4 embodies</rdfs:label>
    <skos:notation>R4</skos:notation>
    <skos:prefLabel xml:lang="en">embodies</skos:prefLabel>
    <rdfs:domain rdf:resource="http://iflastandards.info/ns/lrm/lrmoo/F3_Manifestation"/>
    <rdfs:range rdf:resource="http://iflastandards.info/ns/lrm/lrmoo/F2_Expression"/>
    <owl:inverseOf rdf:resource="http://iflastandards.info/ns/lrm/lrmoo/R4i_is_embodied_in"/>
    <rdfs:subPropertyOf rdf:resource="http://www.cidoc-crm.org/cidoc-crm/P165_incorporates"/>
    <rdfs:comment xml:lang="en">Quantification: many to many, necessary, dependent (1,n:1,n)

Scope note:
This property associates an instance of F3 Manifestation with one or more instances of F2 Expression which are rendered by this instance of F3 Manifestation. The manifestation formats the expression(s) in the way they are to be presented to some public, including specifying the intended sensory impression (such as visual appearance or audio rendition).

Examples:
- The publication ‘Murder on the Orient Express / Agatha Christie’, published by Collins Crime Club in 1934 (F3) embodies the original text in English by Agatha Christie (F2).
- The publication ‘Mord im Orientexpress: ein Hercule-Poirot-Roman / Agatha Christie’, published by Deutscher Bücherbund in 1975 (F3) embodies the German translation by Elisabeth van Bebber (F2).
- The publication ‘The Illustrated Odyssey’, published by Sidgwick &amp; Jackson Ltd in 1980 (F3) embodies the translated text by E. V. Rieu (F2), the introductory text by Jacquetta Hawkes (F2) and photographs by Tim Mercer (F2).
- The publication entitled ‘Alfred Hitchcock’s Psycho: 60th Anniversary Edition’ which was released in 2020 (F3), embodies the original cut of the movie (F2) and the censored version that was released in Britain (F2).
- The publication identified by ISBN ‘2-222-00835-2’ (F3) embodies the text of Marin Mersenne’s ‘Harmonie universelle’ (F2).
- The CD publication ‘Bach Goldberg Variations’ published by Hyperion Records in 2016 (F3), embodies Angela Hewitt’s performances of Bach’s ‘Goldberg Variations’ recorded in Christuskirche (Berlin) on 14-17 December 2015 (F2).
</rdfs:comment>
  </owl:ObjectProperty>
  <owl:ObjectProperty rdf:about="R4i_is_embodied_in">
    <rdfs:label xml:lang="en">R4i is embodied in</rdfs:label>
    <skos:notation>R4i</skos:notation>
    <skos:prefLabel xml:lang="en">is embodied in</skos:prefLabel>
    <rdfs:domain rdf:resource="http://iflastandards.info/ns/lrm/lrmoo/F2_Expression"/>
    <rdfs:range rdf:resource="http://iflastandards.info/ns/lrm/lrmoo/F3_Manifestation"/>
    <owl:inverseOf rdf:resource="http://iflastandards.info/ns/lrm/lrmoo/R4_embodies"/>
    <rdfs:subPropertyOf rdf:resource="http://www.cidoc-crm.org/cidoc-crm/P165i_is_incorporated_in"/>
    <rdfs:comment xml:lang="en">Quantification of the inverse property: many to many, necessary, dependent (1,n:1,n)

Scope note of the inverse property:
This property associates an instance of F3 Manifestation with one or more instances of F2 Expression which are rendered by this instance of F3 Manifestation. The manifestation formats the expression(s) in the way they are to be presented to some public, including specifying the intended sensory impression (such as visual appearance or audio rendition).

Examples of the inverse property:
- The publication ‘Murder on the Orient Express / Agatha Christie’, published by Collins Crime Club in 1934 (F3) embodies the original text in English by Agatha Christie (F2).
- The publication ‘Mord im Orientexpress: ein Hercule-Poirot-Roman / Agatha Christie’, published by Deutscher Bücherbund in 1975 (F3) embodies the German translation by Elisabeth van Bebber (F2).
- The publication ‘The Illustrated Odyssey’, published by Sidgwick &amp; Jackson Ltd in 1980 (F3) embodies the translated text by E. V. Rieu (F2), the introductory text by Jacquetta Hawkes (F2) and photographs by Tim Mercer (F2).
- The publication entitled ‘Alfred Hitchcock’s Psycho: 60th Anniversary Edition’ which was released in 2020 (F3), embodies the original cut of the movie (F2) and the censored version that was released in Britain (F2).
- The publication identified by ISBN ‘2-222-00835-2’ (F3) embodies the text of Marin Mersenne’s ‘Harmonie universelle’ (F2).
- The CD publication ‘Bach Goldberg Variations’ published by Hyperion Records in 2016 (F3), embodies Angela Hewitt’s performances of Bach’s ‘Goldberg Variations’ recorded in Christuskirche (Berlin) on 14-17 December 2015 (F2).
</rdfs:comment>
  </owl:ObjectProperty>
  <owl:ObjectProperty rdf:about="R5_has_component">
    <rdfs:label xml:lang="en">R5 has component</rdfs:label>
    <skos:notation>R5</skos:notation>
    <skos:prefLabel xml:lang="en">has component</skos:prefLabel>
    <rdfs:domain rdf:resource="http://iflastandards.info/ns/lrm/lrmoo/F2_Expression"/>
    <rdfs:range rdf:resource="http://iflastandards.info/ns/lrm/lrmoo/F2_Expression"/>
    <owl:inverseOf rdf:resource="http://iflastandards.info/ns/lrm/lrmoo/R5i_is_component_of"/>
    <rdfs:subPropertyOf rdf:resource="http://www.cidoc-crm.org/cidoc-crm/P148_has_component"/>
    <rdfs:comment xml:lang="en">Quantification: many to many (0,n:0,n)

Scope note:
This property associates an instance of an F2 Expression X with a structural component Y that conveys a part of the overall work realized by X, such as volumes, chapters, or sections. This property is transitive, asymmetric and irreflexive.
Any part of an expression that conveys complete propositions, such as a single phrase, can be documented using the more general property P148 has component (is component of).
Any part of an expression that does not completely follow meaningful boundaries, such as lines or pages of text or portions visible on images, can be documented using the property P106 is composed of (forms part of), and not with R5 has component (is component of). Fragments, in particular, can be documented with the more specific property R15 has fragment (is fragment of).
This property does not cover the relationship that exists between expressions that are realisations of different works, where one is re-used in a new, larger expression. Such a relationship is modelled by R75 incorporates (is incorporated in).

Examples:
- The musical notation for Bach’s ‘Goldberg Variations’ (F2) has component the musical notation for ‘Variatio 1. a 1 Clav’ (F2).
- The Italian text of Dante’s textual work entitled ‘Divina Commedia’ (F2) has component the Italian text of Dante’s textual work entitled ‘Inferno’ (F2).
- The musical notation of Mozart’s Singspiel entitled ‘Die Zauberflöte’ (F2) has component the musical notation of Mozart’s aria entitled ‘Der Hölle Rache’, also known as ‘The Queen of the Night’s Aria’ (F2).
- The visual content of the map entitled ‘Wales – The Midlands – South West England’, scale 1:400,000, issued by Michelin in 2005 (F2) has component the visual content of the inset entitled ‘Liverpool’, scale 1:200,000, set within the compass of the map titled ‘Wales – The Midlands – South West England’, scale 1:400,000, issued by Michelin in 2005 (F2).
</rdfs:comment>
  </owl:ObjectProperty>
  <owl:ObjectProperty rdf:about="R5i_is_component_of">
    <rdfs:label xml:lang="en">R5i is component of</rdfs:label>
    <skos:notation>R5i</skos:notation>
    <skos:prefLabel xml:lang="en">is component of</skos:prefLabel>
    <rdfs:domain rdf:resource="http://iflastandards.info/ns/lrm/lrmoo/F2_Expression"/>
    <rdfs:range rdf:resource="http://iflastandards.info/ns/lrm/lrmoo/F2_Expression"/>
    <owl:inverseOf rdf:resource="http://iflastandards.info/ns/lrm/lrmoo/R5_has_component"/>
    <rdfs:subPropertyOf rdf:resource="http://www.cidoc-crm.org/cidoc-crm/P148i_is_component_of"/>
    <rdfs:comment xml:lang="en">Quantification of the inverse property: many to many (0,n:0,n)

Scope note of the inverse property:
This property associates an instance of an F2 Expression X with a structural component Y that conveys a part of the overall work realized by X, such as volumes, chapters, or sections. This property is transitive, asymmetric and irreflexive.
Any part of an expression that conveys complete propositions, such as a single phrase, can be documented using the more general property P148 has component (is component of).
Any part of an expression that does not completely follow meaningful boundaries, such as lines or pages of text or portions visible on images, can be documented using the property P106 is composed of (forms part of), and not with R5 has component (is component of). Fragments, in particular, can be documented with the more specific property R15 has fragment (is fragment of).
This property does not cover the relationship that exists between expressions that are realisations of different works, where one is re-used in a new, larger expression. Such a relationship is modelled by R75 incorporates (is incorporated in).

Examples of the inverse property:
- The musical notation for Bach’s ‘Goldberg Variations’ (F2) has component the musical notation for ‘Variatio 1. a 1 Clav’ (F2).
- The Italian text of Dante’s textual work entitled ‘Divina Commedia’ (F2) has component the Italian text of Dante’s textual work entitled ‘Inferno’ (F2).
- The musical notation of Mozart’s Singspiel entitled ‘Die Zauberflöte’ (F2) has component the musical notation of Mozart’s aria entitled ‘Der Hölle Rache’, also known as ‘The Queen of the Night’s Aria’ (F2).
- The visual content of the map entitled ‘Wales – The Midlands – South West England’, scale 1:400,000, issued by Michelin in 2005 (F2) has component the visual content of the inset entitled ‘Liverpool’, scale 1:200,000, set within the compass of the map titled ‘Wales – The Midlands – South West England’, scale 1:400,000, issued by Michelin in 2005 (F2).
</rdfs:comment>
  </owl:ObjectProperty>
  <owl:ObjectProperty rdf:about="R7_exemplifies">
    <rdfs:label xml:lang="en">R7 exemplifies</rdfs:label>
    <skos:notation>R7</skos:notation>
    <skos:prefLabel xml:lang="en">exemplifies</skos:prefLabel>
    <rdfs:domain rdf:resource="http://iflastandards.info/ns/lrm/lrmoo/F5_Item"/>
    <rdfs:range rdf:resource="http://iflastandards.info/ns/lrm/lrmoo/F3_Manifestation"/>
    <owl:inverseOf rdf:resource="http://iflastandards.info/ns/lrm/lrmoo/R7i_is_exemplified_by"/>
    <rdfs:subPropertyOf rdf:resource="http://www.cidoc-crm.org/cidoc-crm/P128_carries"/>
    <rdfs:comment xml:lang="en">Quantification: many to one, necessary (1,1:0,n)

Scope note:
This property associates an instance of F3 Manifestation with an instance of F5 Item that is one of its exemplars or its only exemplar.
Instances of F5 Item correspond to the kinds of physical unit(s) specified in the manifestation, regardless of possible later changes.
Even though an item may exhibit defects with respect to the intended manifestation, it is still regarded to carry the manifestation, as long as it is produced or made accessible as a functional item by its creators.

Examples:
- The item held by the Deichman public library in Oslo, identified by inventory number ‘9138513’ (F5) exemplifies the publication ‘Murder on the Orient Express / Agatha Christie’, HarperCollins 2017 (F3).
- The item held by the National Library of France and identified by shelf mark ‘Res 8 P 10’ (F5) exemplifies the edition of Amerigo Vespucci’s textual and cartographic work entitled ‘Mundus novus’ issued in Paris ca. 1503-1504 (F3).
</rdfs:comment>
  </owl:ObjectProperty>
  <owl:ObjectProperty rdf:about="R7i_is_exemplified_by">
    <rdfs:label xml:lang="en">R7i is exemplified by</rdfs:label>
    <skos:notation>R7i</skos:notation>
    <skos:prefLabel xml:lang="en">is exemplified by</skos:prefLabel>
    <rdfs:domain rdf:resource="http://iflastandards.info/ns/lrm/lrmoo/F3_Manifestation"/>
    <rdfs:range rdf:resource="http://iflastandards.info/ns/lrm/lrmoo/F5_Item"/>
    <owl:inverseOf rdf:resource="http://iflastandards.info/ns/lrm/lrmoo/R7_exemplifies"/>
    <rdfs:subPropertyOf rdf:resource="http://www.cidoc-crm.org/cidoc-crm/P128i_is_carried_by"/>
    <rdfs:comment xml:lang="en">Quantification of the inverse property: many to one, necessary (1,1:0,n)

Scope note of the inverse property:
This property associates an instance of F3 Manifestation with an instance of F5 Item that is one of its exemplars or its only exemplar.
Instances of F5 Item correspond to the kinds of physical unit(s) specified in the manifestation, regardless of possible later changes.
Even though an item may exhibit defects with respect to the intended manifestation, it is still regarded to carry the manifestation, as long as it is produced or made accessible as a functional item by its creators.

Examples of the inverse property:
- The item held by the Deichman public library in Oslo, identified by inventory number ‘9138513’ (F5) exemplifies the publication ‘Murder on the Orient Express / Agatha Christie’, HarperCollins 2017 (F3).
- The item held by the National Library of France and identified by shelf mark ‘Res 8 P 10’ (F5) exemplifies the edition of Amerigo Vespucci’s textual and cartographic work entitled ‘Mundus novus’ issued in Paris ca. 1503-1504 (F3).
</rdfs:comment>
  </owl:ObjectProperty>
  <owl:ObjectProperty rdf:about="R8_combines">
    <rdfs:label xml:lang="en">R8 combines</rdfs:label>
    <skos:notation>R8</skos:notation>
    <skos:prefLabel xml:lang="en">combines</skos:prefLabel>
    <rdfs:domain rdf:resource="http://iflastandards.info/ns/lrm/lrmoo/F12_Nomen"/>
    <rdfs:range rdf:resource="http://iflastandards.info/ns/lrm/lrmoo/F12_Nomen"/>
    <owl:inverseOf rdf:resource="http://iflastandards.info/ns/lrm/lrmoo/R8i_is_combined_to_form"/>
    <rdfs:comment xml:lang="en">Quantification: many to many (0,n:0,n)

Shortcut Of: F12 Nomen (1). R33 has string: E62 String (1). P190i is symbolic content of: E90 Symbolic Object (1): P106 is composed of: E90 Symbolic Object (2). P190 has symbolic content: E62 String (2). R33i is string of: F12 Nomen (2)

Scope note:
This property associates an instance of F12 Nomen with another instance of F12 Nomen where the string of the domain instance of F12 Nomen includes the complete symbolic content of the string of the range instance of F12 Nomen. This property is not transitive. It is asymmetric and irreflexive.

Examples:
- ‘The Adoration of the Shepherds (Coventry)’ as a controlled access point for the work (F12) combines ‘The Adoration of the Shepherds’ as the preferred title of the work (F12).
- ‘The Adoration of the Shepherds (Coventry)’ as a controlled access point for the work (F12) combines ‘Coventry’ as a term that refers to a place (F12).
- ‘Guillaume, de Machaut, ca. 1300-1377’ as a controlled access point for the French composer and poet (F12) combines ‘ca. 1300-1377’ as a term that refers to a time-span (F12).
- ‘Guillaume, de Machaut, ca. 1300-1377’ as a controlled access point for the French composer and poet (F12) combines ‘Guillaume de Machaut’ as a name for the person (F12).
- ‘Univerza v Ljubljani. Oddelek za bibliotekarstvo’ as a controlled access point for a corporate body (F12) combines ‘Univerza v Ljubljani’ as a controlled access point for a parent corporate body (F12).
- ‘Univerza v Ljubljani. Oddelek za bibliotekarstvo’ as a controlled access point for a corporate body (F12) combines ‘Oddelek za bibliotekarstvo’ the preferred name that refers to a subordinate corporate body (F12).
- ISBN-10 ‘978-002-002-0’ as an identifier for the publication entitled ‘Nigeria’s international economic relations’ (F12) combines ‘978’ as a code indicating the Nigerian ISBN Agency (F12).
- ISBN-10 ‘978-002-002-0’ as an identifier for the publication entitled ‘Nigeria’s international economic relations’ (F12) combines ‘002’ as a code indicating the Nigerian Institute of International Affairs (F12).
- ISBN-10 ‘978-002-002-0’ as an identifier for the publication entitled ‘Nigeria’s international economic relations’ (F12) combines ‘002’ as a code for the publication entitled ‘Nigeria’s international economic relations’ (F12).
- ‘History -- France -- 14th century’ as a controlled subject term for the concept (F12) combines ‘History’ as the preferred term for the concept (F12). [Subject term constructed according to the order and syntax prescribed in the Library of Congress Subject Headings (LCSH) subject headings language.]
- ‘History -- France -- 14th century’ as a controlled subject term for the concept (F12) combines ‘France’ as the preferred term for the country (F12). [Subject term constructed according to the order and syntax prescribed in the Library of Congress Subject Headings (LCSH) subject headings language.]
- ‘History -- France -- 14th century’ as a controlled subject term for the concept (F12) combines ‘14th century’ as the preferred term for the time-span (F12). [Subject term constructed according to the order and syntax prescribed in the Library of Congress Subject Headings (LCSH) subject headings language.]
- ‘595.7096’ as a classification number for insects in Africa (F12) combines ‘595.7’ as the classification number for the taxonomic class Insecta (insects) (F12). [Classification number according to the 23rd edition of the Dewey Decimal Classification (DDC23).]
- ‘595.7096’ as a classification number for insects in Africa (F12) combines ‘096’ as the notation corresponding to the continent Africa (F12). [Classification number constructed using the geographic regions table in the 23rd edition of the Dewey Decimal Classification (DDC23).]
- ‘Orange (Colour)’ as a controlled subject term for the concept (F12) combines ‘Orange’ the English language term for the colour (F12). [Terms combined according to the syntax of the Art and Architecture Thesaurus (AAT).]
- ‘Orange (Colour)’ as a controlled subject term for the concept (F12) combines ‘Colour’ the English language term for the concept (F12). [Terms combined according to the syntax of the Art and Architecture Thesaurus (AAT).]
</rdfs:comment>
  </owl:ObjectProperty>
  <owl:ObjectProperty rdf:about="R8i_is_combined_to_form">
    <rdfs:label xml:lang="en">R8i is combined to form</rdfs:label>
    <skos:notation>R8i</skos:notation>
    <skos:prefLabel xml:lang="en">is combined to form</skos:prefLabel>
    <rdfs:domain rdf:resource="http://iflastandards.info/ns/lrm/lrmoo/F12_Nomen"/>
    <rdfs:range rdf:resource="http://iflastandards.info/ns/lrm/lrmoo/F12_Nomen"/>
    <owl:inverseOf rdf:resource="http://iflastandards.info/ns/lrm/lrmoo/R8_combines"/>
    <rdfs:comment xml:lang="en">Quantification of the inverse property: many to many (0,n:0,n)

Shortcut Of of the inverse property: F12 Nomen (1). R33 has string: E62 String (1). P190i is symbolic content of: E90 Symbolic Object (1): P106 is composed of: E90 Symbolic Object (2). P190 has symbolic content: E62 String (2). R33i is string of: F12 Nomen (2)

Scope note of the inverse property:
This property associates an instance of F12 Nomen with another instance of F12 Nomen where the string of the domain instance of F12 Nomen includes the complete symbolic content of the string of the range instance of F12 Nomen. This property is not transitive. It is asymmetric and irreflexive.

Examples of the inverse property:
- ‘The Adoration of the Shepherds (Coventry)’ as a controlled access point for the work (F12) combines ‘The Adoration of the Shepherds’ as the preferred title of the work (F12).
- ‘The Adoration of the Shepherds (Coventry)’ as a controlled access point for the work (F12) combines ‘Coventry’ as a term that refers to a place (F12).
- ‘Guillaume, de Machaut, ca. 1300-1377’ as a controlled access point for the French composer and poet (F12) combines ‘ca. 1300-1377’ as a term that refers to a time-span (F12).
- ‘Guillaume, de Machaut, ca. 1300-1377’ as a controlled access point for the French composer and poet (F12) combines ‘Guillaume de Machaut’ as a name for the person (F12).
- ‘Univerza v Ljubljani. Oddelek za bibliotekarstvo’ as a controlled access point for a corporate body (F12) combines ‘Univerza v Ljubljani’ as a controlled access point for a parent corporate body (F12).
- ‘Univerza v Ljubljani. Oddelek za bibliotekarstvo’ as a controlled access point for a corporate body (F12) combines ‘Oddelek za bibliotekarstvo’ the preferred name that refers to a subordinate corporate body (F12).
- ISBN-10 ‘978-002-002-0’ as an identifier for the publication entitled ‘Nigeria’s international economic relations’ (F12) combines ‘978’ as a code indicating the Nigerian ISBN Agency (F12).
- ISBN-10 ‘978-002-002-0’ as an identifier for the publication entitled ‘Nigeria’s international economic relations’ (F12) combines ‘002’ as a code indicating the Nigerian Institute of International Affairs (F12).
- ISBN-10 ‘978-002-002-0’ as an identifier for the publication entitled ‘Nigeria’s international economic relations’ (F12) combines ‘002’ as a code for the publication entitled ‘Nigeria’s international economic relations’ (F12).
- ‘History -- France -- 14th century’ as a controlled subject term for the concept (F12) combines ‘History’ as the preferred term for the concept (F12). [Subject term constructed according to the order and syntax prescribed in the Library of Congress Subject Headings (LCSH) subject headings language.]
- ‘History -- France -- 14th century’ as a controlled subject term for the concept (F12) combines ‘France’ as the preferred term for the country (F12). [Subject term constructed according to the order and syntax prescribed in the Library of Congress Subject Headings (LCSH) subject headings language.]
- ‘History -- France -- 14th century’ as a controlled subject term for the concept (F12) combines ‘14th century’ as the preferred term for the time-span (F12). [Subject term constructed according to the order and syntax prescribed in the Library of Congress Subject Headings (LCSH) subject headings language.]
- ‘595.7096’ as a classification number for insects in Africa (F12) combines ‘595.7’ as the classification number for the taxonomic class Insecta (insects) (F12). [Classification number according to the 23rd edition of the Dewey Decimal Classification (DDC23).]
- ‘595.7096’ as a classification number for insects in Africa (F12) combines ‘096’ as the notation corresponding to the continent Africa (F12). [Classification number constructed using the geographic regions table in the 23rd edition of the Dewey Decimal Classification (DDC23).]
- ‘Orange (Colour)’ as a controlled subject term for the concept (F12) combines ‘Orange’ the English language term for the colour (F12). [Terms combined according to the syntax of the Art and Architecture Thesaurus (AAT).]
- ‘Orange (Colour)’ as a controlled subject term for the concept (F12) combines ‘Colour’ the English language term for the concept (F12). [Terms combined according to the syntax of the Art and Architecture Thesaurus (AAT).]
</rdfs:comment>
  </owl:ObjectProperty>
  <owl:ObjectProperty rdf:about="R10_is_member_of">
    <rdfs:label xml:lang="en">R10 is member of</rdfs:label>
    <skos:notation>R10</skos:notation>
    <skos:prefLabel xml:lang="en">is member of</skos:prefLabel>
    <rdfs:domain rdf:resource="http://iflastandards.info/ns/lrm/lrmoo/F1_Work"/>
    <rdfs:range rdf:resource="http://www.cidoc-crm.org/cidoc-crm/E28_Conceptual_Object"/>
    <owl:inverseOf rdf:resource="http://iflastandards.info/ns/lrm/lrmoo/R10i_has_member"/>
    <rdfs:comment xml:lang="en">Quantification: many to many (0,n:0,n)

Scope note:
This property associates an instance of F1 Work with an instance of E28 Conceptual Object that represents a generalization of the work. The property can be used to group variant, alternative or related works that are considered to share a common concept.
Whereas instances of F1 Work are always realised in instances of F2 Expression, there is no particular expression that fully conveys the instance of Conceptual Object that a work may be a member of.
Intended usage of the property includes what is discussed as “superwork” in the library community. Typical examples are novels that can be grouped by fictional universes or common characters, paintings or graphical works that exist as a family of alternatives, musical compositions that are referred to as the same although they exist as particular versions that are each identified as an individual work. The instance of E28 Conceptual Object that has works as members will often be constructed for a specific purpose, such as bibliographic organization or retrieval.

Examples:
- Auguste Rodin’s ‘Le penseur’ (E28) has member Auguste Rodin’s ‘Le penseur’ in monumental size (F1). [In original size this sculpture forms part of (R67i) Rodin’s ‘La Porte de l’Enfer’ (F1); in monumental size it is an autonomous work. All scale variants are members of (R10) the superwork ‘Le penseur’(E28).]
- Edward Munch’s ‘Madonna’ (E28) has member Edward Munch’s black and white graphical work ‘Madonna’ (F1).
- Edward Munch’s ‘Madonna’ (E28) has member Edward Munch’s painting ‘Madonna’ (F1).
- Ludwig van Beethoven’s opera Op. 72 ‘Fidelio’ (E28) has member Ludwig van Beethoven’s opera ‘Leonore, oder Der Triumph der ehelichen Liebe’ (the initial version that was performed in 1805) (F1).
- Ludwig van Beethoven’s opera Op. 72 ‘Fidelio’ (E28) has member Ludwig van Beethoven’s opera ‘Fidelio’ (the final version that was first performed in 1814) (F1).
- The fictional universe created by Terry Pratchett referred to as ‘Discworld’ (E28) has member Terry Pratchett’s novel ‘The Light Fantastic’ (F1).
- The fictional universe created by Terry Pratchett referred to as ‘Discworld’ (E28) has member ‘Where’s my Cow’, a picture book by Terry Pratchett and Melvyn Grant (F1).
</rdfs:comment>
  </owl:ObjectProperty>
  <owl:ObjectProperty rdf:about="R10i_has_member">
    <rdfs:label xml:lang="en">R10i has member</rdfs:label>
    <skos:notation>R10i</skos:notation>
    <skos:prefLabel xml:lang="en">has member</skos:prefLabel>
    <rdfs:domain rdf:resource="http://www.cidoc-crm.org/cidoc-crm/E28_Conceptual_Object"/>
    <rdfs:range rdf:resource="http://iflastandards.info/ns/lrm/lrmoo/F1_Work"/>
    <owl:inverseOf rdf:resource="http://iflastandards.info/ns/lrm/lrmoo/R10_is_member_of"/>
    <rdfs:comment xml:lang="en">Quantification of the inverse property: many to many (0,n:0,n)

Scope note of the inverse property:
This property associates an instance of F1 Work with an instance of E28 Conceptual Object that represents a generalization of the work. The property can be used to group variant, alternative or related works that are considered to share a common concept.
Whereas instances of F1 Work are always realised in instances of F2 Expression, there is no particular expression that fully conveys the instance of Conceptual Object that a work may be a member of.
Intended usage of the property includes what is discussed as “superwork” in the library community. Typical examples are novels that can be grouped by fictional universes or common characters, paintings or graphical works that exist as a family of alternatives, musical compositions that are referred to as the same although they exist as particular versions that are each identified as an individual work. The instance of E28 Conceptual Object that has works as members will often be constructed for a specific purpose, such as bibliographic organization or retrieval.

Examples of the inverse property:
- Auguste Rodin’s ‘Le penseur’ (E28) has member Auguste Rodin’s ‘Le penseur’ in monumental size (F1). [In original size this sculpture forms part of (R67i) Rodin’s ‘La Porte de l’Enfer’ (F1); in monumental size it is an autonomous work. All scale variants are members of (R10) the superwork ‘Le penseur’(E28).]
- Edward Munch’s ‘Madonna’ (E28) has member Edward Munch’s black and white graphical work ‘Madonna’ (F1).
- Edward Munch’s ‘Madonna’ (E28) has member Edward Munch’s painting ‘Madonna’ (F1).
- Ludwig van Beethoven’s opera Op. 72 ‘Fidelio’ (E28) has member Ludwig van Beethoven’s opera ‘Leonore, oder Der Triumph der ehelichen Liebe’ (the initial version that was performed in 1805) (F1).
- Ludwig van Beethoven’s opera Op. 72 ‘Fidelio’ (E28) has member Ludwig van Beethoven’s opera ‘Fidelio’ (the final version that was first performed in 1814) (F1).
- The fictional universe created by Terry Pratchett referred to as ‘Discworld’ (E28) has member Terry Pratchett’s novel ‘The Light Fantastic’ (F1).
- The fictional universe created by Terry Pratchett referred to as ‘Discworld’ (E28) has member ‘Where’s my Cow’, a picture book by Terry Pratchett and Melvyn Grant (F1).
</rdfs:comment>
  </owl:ObjectProperty>
  <owl:ObjectProperty rdf:about="R11_has_issuing_rule">
    <rdfs:label xml:lang="en">R11 has issuing rule</rdfs:label>
    <skos:notation>R11</skos:notation>
    <skos:prefLabel xml:lang="en">has issuing rule</skos:prefLabel>
    <rdfs:domain rdf:resource="http://iflastandards.info/ns/lrm/lrmoo/F18_Serial_Work"/>
    <rdfs:range rdf:resource="http://www.cidoc-crm.org/cidoc-crm/E29_Design_or_Procedure"/>
    <owl:inverseOf rdf:resource="http://iflastandards.info/ns/lrm/lrmoo/R11i_is_issuing_rule_of"/>
    <rdfs:comment xml:lang="en">Quantification: many to many (0,n:0,n)

Shortcut Of: F18 Serial Work. R19i was realised through: F30 Manifestation Creation. P16 used specific object (was used for): E29 Design or Procedure

Scope note:
This property associates an instance of F18 Serial Work with the instance of E29 Design or Procedure that specifies the issuing policy planned by this instance of F18 Serial Work, such as sequencing pattern, expected frequency and expected regularity.

Examples:
- [Editor’s note: Transfer this property to PRESS(OO) once version 2.0 has a stable draft. Implement this property only in conjunction with an implementation of PRESS(OO).]
- The serial entitled ‘Quarterly journal of pure and applied mathematics’, identified by ISSN ‘1549-6724’ (F18) has issuing rule to be issued every three months, on a regular basis, with each issue being numbered according to the pattern ‘Vol. 1, no. 1 (2005)’ that was observed by the Library of Congress’s cataloguers on an exemplar of the first issue (E29).
</rdfs:comment>
  </owl:ObjectProperty>
  <owl:ObjectProperty rdf:about="R11i_is_issuing_rule_of">
    <rdfs:label xml:lang="en">R11i is issuing rule of</rdfs:label>
    <skos:notation>R11i</skos:notation>
    <skos:prefLabel xml:lang="en">is issuing rule of</skos:prefLabel>
    <rdfs:domain rdf:resource="http://www.cidoc-crm.org/cidoc-crm/E29_Design_or_Procedure"/>
    <rdfs:range rdf:resource="http://iflastandards.info/ns/lrm/lrmoo/F18_Serial_Work"/>
    <owl:inverseOf rdf:resource="http://iflastandards.info/ns/lrm/lrmoo/R11_has_issuing_rule"/>
    <rdfs:comment xml:lang="en">Quantification of the inverse property: many to many (0,n:0,n)

Shortcut Of of the inverse property: F18 Serial Work. R19i was realised through: F30 Manifestation Creation. P16 used specific object (was used for): E29 Design or Procedure

Scope note of the inverse property:
This property associates an instance of F18 Serial Work with the instance of E29 Design or Procedure that specifies the issuing policy planned by this instance of F18 Serial Work, such as sequencing pattern, expected frequency and expected regularity.

Examples of the inverse property:
- [Editor’s note: Transfer this property to PRESS(OO) once version 2.0 has a stable draft. Implement this property only in conjunction with an implementation of PRESS(OO).]
- The serial entitled ‘Quarterly journal of pure and applied mathematics’, identified by ISSN ‘1549-6724’ (F18) has issuing rule to be issued every three months, on a regular basis, with each issue being numbered according to the pattern ‘Vol. 1, no. 1 (2005)’ that was observed by the Library of Congress’s cataloguers on an exemplar of the first issue (E29).
</rdfs:comment>
  </owl:ObjectProperty>
  <owl:ObjectProperty rdf:about="R15_has_fragment">
    <rdfs:label xml:lang="en">R15 has fragment</rdfs:label>
    <skos:notation>R15</skos:notation>
    <skos:prefLabel xml:lang="en">has fragment</skos:prefLabel>
    <rdfs:domain rdf:resource="http://iflastandards.info/ns/lrm/lrmoo/F2_Expression"/>
    <rdfs:range rdf:resource="http://www.cidoc-crm.org/cidoc-crm/E90_Symbolic_Object"/>
    <owl:inverseOf rdf:resource="http://iflastandards.info/ns/lrm/lrmoo/R15i_is_fragment_of"/>
    <rdfs:subPropertyOf rdf:resource="http://www.cidoc-crm.org/cidoc-crm/P106_is_composed_of"/>
    <rdfs:comment xml:lang="en">Quantification: many to many (0,n:0,n)

Scope note:
This property associates an instance of E90 Symbolic Object with an instance of F2 Expression of which it is a fragment. The fragment is not itself an instance of F2 Expression as it does not express any instance of F1 Work. When the fragment consists of intelligible words it is an instance of E33 Linguistic Object.
An instance of E90 Symbolic Object is only considered a fragment of an instance of F2 Expression when related to its occurrence in a known or assumed whole by the R15 has fragment (is fragment of) property. The size of an instance of E90 Symbolic Object ranges from more than 99% of an instance of F2 Expression to tiny bits (a few words from a text, one bar from a musical composition, one detail from a still image, a two-second clip from a video, etc.).
An instance of E90 Symbolic Object can become a fragment of an instance of F2 Expression through the deterioration over time of a carrier of the expression, such as when only fragments of a manuscript of an ancient text survive. Typically instances of E90 Symbolic Object that are of interest as fragments of expressions are formed deliberately, such as when excerpts are taken from a text by the compiler of a collection of excerpts, or citations from one expression are used in another text.

Examples:
- The ancient Greek text of the four stanzas from an ode by Sappho (E33) that were quoted by Pseudo-Longinus in his textual work entitled ‘On the sublime’ is fragment of the complete ancient Greek text, now irremediably lost, of Sappho’s ode currently identified as Sappho’s poem #2 (F2).
- The phrase ‘Beati pauperes spiritu’ (E33) is fragment of the Latin text of the Gospel according to St. Matthew (F2). [excerpt from Matthew 5,3]
- The stanza ‘Nel mezzo del cammin di nostra vita / mi ritrovai per una selva oscura / ché la diritta via era smarrita’ (E33) is fragment of the Italian text of Dante Alighieri’s ‘Inferno’ from the ‘Divina Commedia’ (F2).
- The widely recognized ominous four-note opening motif (E73) is fragment of Beethoven’s Fifth Symphony (F2).
- The melting clock (E36) is fragment of the painting ‘Persistence of Memory’ by Salvador Dali, 1931 (F2).
</rdfs:comment>
  </owl:ObjectProperty>
  <owl:ObjectProperty rdf:about="R15i_is_fragment_of">
    <rdfs:label xml:lang="en">R15i is fragment of</rdfs:label>
    <skos:notation>R15i</skos:notation>
    <skos:prefLabel xml:lang="en">is fragment of</skos:prefLabel>
    <rdfs:domain rdf:resource="http://www.cidoc-crm.org/cidoc-crm/E90_Symbolic_Object"/>
    <rdfs:range rdf:resource="http://iflastandards.info/ns/lrm/lrmoo/F2_Expression"/>
    <owl:inverseOf rdf:resource="http://iflastandards.info/ns/lrm/lrmoo/R15_has_fragment"/>
    <rdfs:subPropertyOf rdf:resource="http://www.cidoc-crm.org/cidoc-crm/P106i_forms_part_of"/>
    <rdfs:comment xml:lang="en">Quantification of the inverse property: many to many (0,n:0,n)

Scope note of the inverse property:
This property associates an instance of E90 Symbolic Object with an instance of F2 Expression of which it is a fragment. The fragment is not itself an instance of F2 Expression as it does not express any instance of F1 Work. When the fragment consists of intelligible words it is an instance of E33 Linguistic Object.
An instance of E90 Symbolic Object is only considered a fragment of an instance of F2 Expression when related to its occurrence in a known or assumed whole by the R15 has fragment (is fragment of) property. The size of an instance of E90 Symbolic Object ranges from more than 99% of an instance of F2 Expression to tiny bits (a few words from a text, one bar from a musical composition, one detail from a still image, a two-second clip from a video, etc.).
An instance of E90 Symbolic Object can become a fragment of an instance of F2 Expression through the deterioration over time of a carrier of the expression, such as when only fragments of a manuscript of an ancient text survive. Typically instances of E90 Symbolic Object that are of interest as fragments of expressions are formed deliberately, such as when excerpts are taken from a text by the compiler of a collection of excerpts, or citations from one expression are used in another text.

Examples of the inverse property:
- The ancient Greek text of the four stanzas from an ode by Sappho (E33) that were quoted by Pseudo-Longinus in his textual work entitled ‘On the sublime’ is fragment of the complete ancient Greek text, now irremediably lost, of Sappho’s ode currently identified as Sappho’s poem #2 (F2).
- The phrase ‘Beati pauperes spiritu’ (E33) is fragment of the Latin text of the Gospel according to St. Matthew (F2). [excerpt from Matthew 5,3]
- The stanza ‘Nel mezzo del cammin di nostra vita / mi ritrovai per una selva oscura / ché la diritta via era smarrita’ (E33) is fragment of the Italian text of Dante Alighieri’s ‘Inferno’ from the ‘Divina Commedia’ (F2).
- The widely recognized ominous four-note opening motif (E73) is fragment of Beethoven’s Fifth Symphony (F2).
- The melting clock (E36) is fragment of the painting ‘Persistence of Memory’ by Salvador Dali, 1931 (F2).
</rdfs:comment>
  </owl:ObjectProperty>
  <owl:ObjectProperty rdf:about="R16_created">
    <rdfs:label xml:lang="en">R16 created</rdfs:label>
    <skos:notation>R16</skos:notation>
    <skos:prefLabel xml:lang="en">created</skos:prefLabel>
    <rdfs:domain rdf:resource="http://iflastandards.info/ns/lrm/lrmoo/F27_Work_Creation"/>
    <rdfs:range rdf:resource="http://iflastandards.info/ns/lrm/lrmoo/F1_Work"/>
    <owl:inverseOf rdf:resource="http://iflastandards.info/ns/lrm/lrmoo/R16i_was_created_by"/>
    <rdfs:subPropertyOf rdf:resource="http://www.cidoc-crm.org/cidoc-crm/P94_has_created"/>
    <rdfs:comment xml:lang="en">Quantification: one to many, necessary, dependent (1,n:1,1)

Scope note:
This property associates the initial creation of a work and the instance of F1 Work that was created.

Examples:
- Agatha Christie creating ‘Murder on the Orient Express’ (F27), created the work ‘Murder on the Orient Express’ (F1).
- Mary Shelley creating ‘Frankenstein, or, The Modern Prometheus’ (F27), created the work ‘Frankenstein, or, The Modern Prometheus’ (F1).
- Dante creating the poem ‘Divina Commedia’ (F27), created the work ‘Divina Commedia’ (F1).
- William Shakespeare creating ‘The Tragedy of Hamlet, Prince of Denmark’(F27), created the work ‘The Tragedy of Hamlet, Prince of Denmark’ (F1).
- René Goscinny and Albert Uderzo (collaboratively) creating ‘Astérix le Gaulois’ (F27) created the work ‘Astérix le Gaulois’ (F1).
- The work creation event of Ludwig van Beethoven composing his ‘Symphony No. 9’ (F27) created the work ‘Beethoven’s Symphony No. 9’ (F1).
- Johann Sebastian Bach composing the ‘Goldberg Variations’ (F27) created the work the ‘Goldberg Variations’ (F1).
- The making of ‘Jules et Jim’, directed by François Truffault (F27) created the work ‘Jules et Jim’ (F1).
- The making of ‘Psycho’, directed by Alfred Hitchcock (F27) created the work ‘Psycho’ (F1).
- Auguste Rodin creating ‘Le Penseur’ (The Thinker) (F27), created the work ‘Le Penseur’ (The Thinker) (F1).
- Picasso creating ‘Guernica’ (F27) created the work ‘Guernica’ (F1).
</rdfs:comment>
  </owl:ObjectProperty>
  <owl:ObjectProperty rdf:about="R16i_was_created_by">
    <rdfs:label xml:lang="en">R16i was created by</rdfs:label>
    <skos:notation>R16i</skos:notation>
    <skos:prefLabel xml:lang="en">was created by</skos:prefLabel>
    <rdfs:domain rdf:resource="http://iflastandards.info/ns/lrm/lrmoo/F1_Work"/>
    <rdfs:range rdf:resource="http://iflastandards.info/ns/lrm/lrmoo/F27_Work_Creation"/>
    <owl:inverseOf rdf:resource="http://iflastandards.info/ns/lrm/lrmoo/R16_created"/>
    <rdfs:subPropertyOf rdf:resource="http://www.cidoc-crm.org/cidoc-crm/P94i_was_created_by"/>
    <rdfs:comment xml:lang="en">Quantification of the inverse property: one to many, necessary, dependent (1,n:1,1)

Scope note of the inverse property:
This property associates the initial creation of a work and the instance of F1 Work that was created.

Examples of the inverse property:
- Agatha Christie creating ‘Murder on the Orient Express’ (F27), created the work ‘Murder on the Orient Express’ (F1).
- Mary Shelley creating ‘Frankenstein, or, The Modern Prometheus’ (F27), created the work ‘Frankenstein, or, The Modern Prometheus’ (F1).
- Dante creating the poem ‘Divina Commedia’ (F27), created the work ‘Divina Commedia’ (F1).
- William Shakespeare creating ‘The Tragedy of Hamlet, Prince of Denmark’(F27), created the work ‘The Tragedy of Hamlet, Prince of Denmark’ (F1).
- René Goscinny and Albert Uderzo (collaboratively) creating ‘Astérix le Gaulois’ (F27) created the work ‘Astérix le Gaulois’ (F1).
- The work creation event of Ludwig van Beethoven composing his ‘Symphony No. 9’ (F27) created the work ‘Beethoven’s Symphony No. 9’ (F1).
- Johann Sebastian Bach composing the ‘Goldberg Variations’ (F27) created the work the ‘Goldberg Variations’ (F1).
- The making of ‘Jules et Jim’, directed by François Truffault (F27) created the work ‘Jules et Jim’ (F1).
- The making of ‘Psycho’, directed by Alfred Hitchcock (F27) created the work ‘Psycho’ (F1).
- Auguste Rodin creating ‘Le Penseur’ (The Thinker) (F27), created the work ‘Le Penseur’ (The Thinker) (F1).
- Picasso creating ‘Guernica’ (F27) created the work ‘Guernica’ (F1).
</rdfs:comment>
  </owl:ObjectProperty>
  <owl:ObjectProperty rdf:about="R17_created">
    <rdfs:label xml:lang="en">R17 created</rdfs:label>
    <skos:notation>R17</skos:notation>
    <skos:prefLabel xml:lang="en">created</skos:prefLabel>
    <rdfs:domain rdf:resource="http://iflastandards.info/ns/lrm/lrmoo/F28_Expression_Creation"/>
    <rdfs:range rdf:resource="http://iflastandards.info/ns/lrm/lrmoo/F2_Expression"/>
    <owl:inverseOf rdf:resource="http://iflastandards.info/ns/lrm/lrmoo/R17i_was_created_by"/>
    <rdfs:subPropertyOf rdf:resource="http://www.cidoc-crm.org/cidoc-crm/P94_has_created"/>
    <rdfs:comment xml:lang="en">Quantification: one to many, necessary, dependent (1,n:1,1)

Scope note:
This property associates an instance of F2 Expression that was externalised during a particular instance of F28 Expression Creation event with that particular creation event. An instance of expression creation creates an instance of expression and also creates any expressions that are parts of that expression.

Examples:
- Agatha Christie creating the text for her novel ‘Murder on the Orient Express’ (F28) created the original English text of Agatha Christie’s ‘Murder on the Orient Express’ (F2).
- Elisabeth van Bebber creating the text of her translation of Agatha Christie’s ‘Murder on the Orient Express’ (F28) created the German text of Agatha Christie’s ‘Murder on the Orient Express’ (F2).
- Ludwig van Beethoven composing his ‘Symphony No. 9’ (F28) created the original score for the 9th Symphony (F2).
- The making of the censored version of Hitchcock’s movie ‘Psycho’ (F28) created the original version (cut) of the movie that was released in Britain (F2).
- The making of the first plaster version of ‘The Thinker’ sculpture by Auguste Rodin (F28) created the plaster version of ‘The Thinker’ (F2).
- The making of the large-scale version of ‘The Thinker’ by the Fonderie Alexis Rudier in 1904 (F28) created the large-scale version of ‘The Thinker’ (F2).
</rdfs:comment>
  </owl:ObjectProperty>
  <owl:ObjectProperty rdf:about="R17i_was_created_by">
    <rdfs:label xml:lang="en">R17i was created by</rdfs:label>
    <skos:notation>R17i</skos:notation>
    <skos:prefLabel xml:lang="en">was created by</skos:prefLabel>
    <rdfs:domain rdf:resource="http://iflastandards.info/ns/lrm/lrmoo/F2_Expression"/>
    <rdfs:range rdf:resource="http://iflastandards.info/ns/lrm/lrmoo/F28_Expression_Creation"/>
    <owl:inverseOf rdf:resource="http://iflastandards.info/ns/lrm/lrmoo/R17_created"/>
    <rdfs:subPropertyOf rdf:resource="http://www.cidoc-crm.org/cidoc-crm/P94i_was_created_by"/>
    <rdfs:comment xml:lang="en">Quantification of the inverse property: one to many, necessary, dependent (1,n:1,1)

Scope note of the inverse property:
This property associates an instance of F2 Expression that was externalised during a particular instance of F28 Expression Creation event with that particular creation event. An instance of expression creation creates an instance of expression and also creates any expressions that are parts of that expression.

Examples of the inverse property:
- Agatha Christie creating the text for her novel ‘Murder on the Orient Express’ (F28) created the original English text of Agatha Christie’s ‘Murder on the Orient Express’ (F2).
- Elisabeth van Bebber creating the text of her translation of Agatha Christie’s ‘Murder on the Orient Express’ (F28) created the German text of Agatha Christie’s ‘Murder on the Orient Express’ (F2).
- Ludwig van Beethoven composing his ‘Symphony No. 9’ (F28) created the original score for the 9th Symphony (F2).
- The making of the censored version of Hitchcock’s movie ‘Psycho’ (F28) created the original version (cut) of the movie that was released in Britain (F2).
- The making of the first plaster version of ‘The Thinker’ sculpture by Auguste Rodin (F28) created the plaster version of ‘The Thinker’ (F2).
- The making of the large-scale version of ‘The Thinker’ by the Fonderie Alexis Rudier in 1904 (F28) created the large-scale version of ‘The Thinker’ (F2).
</rdfs:comment>
  </owl:ObjectProperty>
  <owl:ObjectProperty rdf:about="R19_created_a_realisation_of">
    <rdfs:label xml:lang="en">R19 created a realisation of</rdfs:label>
    <skos:notation>R19</skos:notation>
    <skos:prefLabel xml:lang="en">created a realisation of</skos:prefLabel>
    <rdfs:domain rdf:resource="http://iflastandards.info/ns/lrm/lrmoo/F28_Expression_Creation"/>
    <rdfs:range rdf:resource="http://iflastandards.info/ns/lrm/lrmoo/F1_Work"/>
    <owl:inverseOf rdf:resource="http://iflastandards.info/ns/lrm/lrmoo/R19i_was_realised_through"/>
    <rdfs:subPropertyOf rdf:resource="http://www.cidoc-crm.org/cidoc-crm/P16_used_specific_object"/>
    <rdfs:comment xml:lang="en">Quantification: many to one, necessary, dependent (1,1:1,n)

Scope note:
This property associates an instance of F28 Expression Creation with the instance of F1 Work which was externalised in an instance of F2 Expression created by this creation event.

Examples:
- Agatha Christie writing the text for her novel ‘Murder on the Orient Express’ (F28) created a realization of Agatha Christie’s ‘Murder on the Orient Express’ (F1).
- Elisabeth van Bebber creating the text of her translation of Agatha Christie’s ‘Murder on the Orient Express’ (F28) created a realization of Agatha Christie’s ‘Murder on the Orient Express’ (F1).
- Ludwig van Beethoven composing his 9th symphony (F28) created a realization of Beethoven’s ‘Symphony No. 9’ (F1).
- The making of the censored version of Hitchcock’s movie ‘Psycho’ (F28) created a realization of Hitchcock’s movie ‘Psycho’ (F1).
- Auguste Rodin making the first plaster version of ‘The Thinker’ sculpture (F28) created a realization of Auguste Rodin’s ‘The Thinker’ (F1).
- The making of the large-scale version of ‘The Thinker’ by the Fonderie Alexis Rudier in 1904 (F28) created a realization of Auguste Rodin’s ‘The Thinker’ (F1).
</rdfs:comment>
  </owl:ObjectProperty>
  <owl:ObjectProperty rdf:about="R19i_was_realised_through">
    <rdfs:label xml:lang="en">R19i was realised through</rdfs:label>
    <skos:notation>R19i</skos:notation>
    <skos:prefLabel xml:lang="en">was realised through</skos:prefLabel>
    <rdfs:domain rdf:resource="http://iflastandards.info/ns/lrm/lrmoo/F1_Work"/>
    <rdfs:range rdf:resource="http://iflastandards.info/ns/lrm/lrmoo/F28_Expression_Creation"/>
    <owl:inverseOf rdf:resource="http://iflastandards.info/ns/lrm/lrmoo/R19_created_a_realisation_of"/>
    <rdfs:subPropertyOf rdf:resource="http://www.cidoc-crm.org/cidoc-crm/P16i_was_used_for"/>
    <rdfs:comment xml:lang="en">Quantification of the inverse property: many to one, necessary, dependent (1,1:1,n)

Scope note of the inverse property:
This property associates an instance of F28 Expression Creation with the instance of F1 Work which was externalised in an instance of F2 Expression created by this creation event.

Examples of the inverse property:
- Agatha Christie writing the text for her novel ‘Murder on the Orient Express’ (F28) created a realization of Agatha Christie’s ‘Murder on the Orient Express’ (F1).
- Elisabeth van Bebber creating the text of her translation of Agatha Christie’s ‘Murder on the Orient Express’ (F28) created a realization of Agatha Christie’s ‘Murder on the Orient Express’ (F1).
- Ludwig van Beethoven composing his 9th symphony (F28) created a realization of Beethoven’s ‘Symphony No. 9’ (F1).
- The making of the censored version of Hitchcock’s movie ‘Psycho’ (F28) created a realization of Hitchcock’s movie ‘Psycho’ (F1).
- Auguste Rodin making the first plaster version of ‘The Thinker’ sculpture (F28) created a realization of Auguste Rodin’s ‘The Thinker’ (F1).
- The making of the large-scale version of ‘The Thinker’ by the Fonderie Alexis Rudier in 1904 (F28) created a realization of Auguste Rodin’s ‘The Thinker’ (F1).
</rdfs:comment>
  </owl:ObjectProperty>
  <owl:ObjectProperty rdf:about="R24_created">
    <rdfs:label xml:lang="en">R24 created</rdfs:label>
    <skos:notation>R24</skos:notation>
    <skos:prefLabel xml:lang="en">created</skos:prefLabel>
    <rdfs:domain rdf:resource="http://iflastandards.info/ns/lrm/lrmoo/F30_Manifestation_Creation"/>
    <rdfs:range rdf:resource="http://iflastandards.info/ns/lrm/lrmoo/F3_Manifestation"/>
    <owl:inverseOf rdf:resource="http://iflastandards.info/ns/lrm/lrmoo/R24i_was_created_through"/>
    <rdfs:subPropertyOf rdf:resource="http://www.cidoc-crm.org/cidoc-crm/P94_has_created"/>
    <rdfs:comment xml:lang="en">Quantification: one to many, necessary, dependent (1,n:1,1)

Scope note:
This property associates the instance of F3 Manifestation that was created during a particular instance of F30 Manifestation Creation with that instance of F30 Manifestation Creation event.

Examples:
- The process of creating the publication ‘Murder on the Orient Express / Agatha Christie’ as published by HarperCollins in 2017 (F30) created ‘Murder on the Orient Express / Agatha Christie’ published by HarperCollins in 2017 (F3).
- The process of making the HTML-version of the English text of Homer’s ‘Odyssey’ (as available online from the Gutenberg Project) (F30) created the HTML-version of the English text of Homer’s ‘Odyssey’ (F3).
- The process of making the CD publication ‘Bach Goldberg Variations’ (as published by Hyperion Records in 2016) (F30) created ‘Bach Goldberg Variations’, published by Hyperion Records in 2016 (F3).
</rdfs:comment>
  </owl:ObjectProperty>
  <owl:ObjectProperty rdf:about="R24i_was_created_through">
    <rdfs:label xml:lang="en">R24i was created through</rdfs:label>
    <skos:notation>R24i</skos:notation>
    <skos:prefLabel xml:lang="en">was created through</skos:prefLabel>
    <rdfs:domain rdf:resource="http://iflastandards.info/ns/lrm/lrmoo/F3_Manifestation"/>
    <rdfs:range rdf:resource="http://iflastandards.info/ns/lrm/lrmoo/F30_Manifestation_Creation"/>
    <owl:inverseOf rdf:resource="http://iflastandards.info/ns/lrm/lrmoo/R24_created"/>
    <rdfs:subPropertyOf rdf:resource="http://www.cidoc-crm.org/cidoc-crm/P94i_was_created_by"/>
    <rdfs:comment xml:lang="en">Quantification of the inverse property: one to many, necessary, dependent (1,n:1,1)

Scope note of the inverse property:
This property associates the instance of F3 Manifestation that was created during a particular instance of F30 Manifestation Creation with that instance of F30 Manifestation Creation event.

Examples of the inverse property:
- The process of creating the publication ‘Murder on the Orient Express / Agatha Christie’ as published by HarperCollins in 2017 (F30) created ‘Murder on the Orient Express / Agatha Christie’ published by HarperCollins in 2017 (F3).
- The process of making the HTML-version of the English text of Homer’s ‘Odyssey’ (as available online from the Gutenberg Project) (F30) created the HTML-version of the English text of Homer’s ‘Odyssey’ (F3).
- The process of making the CD publication ‘Bach Goldberg Variations’ (as published by Hyperion Records in 2016) (F30) created ‘Bach Goldberg Variations’, published by Hyperion Records in 2016 (F3).
</rdfs:comment>
  </owl:ObjectProperty>
  <owl:ObjectProperty rdf:about="R27_materialized">
    <rdfs:label xml:lang="en">R27 materialized</rdfs:label>
    <skos:notation>R27</skos:notation>
    <skos:prefLabel xml:lang="en">materialized</skos:prefLabel>
    <rdfs:domain rdf:resource="http://iflastandards.info/ns/lrm/lrmoo/F32_Item_Production_Event"/>
    <rdfs:range rdf:resource="http://iflastandards.info/ns/lrm/lrmoo/F3_Manifestation"/>
    <owl:inverseOf rdf:resource="http://iflastandards.info/ns/lrm/lrmoo/R27i_was_materialized_by"/>
    <rdfs:subPropertyOf rdf:resource="http://www.cidoc-crm.org/cidoc-crm/P16_used_specific_object"/>
    <rdfs:comment xml:lang="en">Quantification: many to many (0,n:0,n)

Scope note:
This property associates an instance of F32 Item Production Event with the set of signs provided by the publisher to be carried by all of the produced items (i.e., the instances of F5 Item) and any other physical features foreseen as integral to the instance of F3 Manifestation that is materialised.

Examples:
- The production of copies of the paperback edition of the HarperCollins 2017 publication ‘Murder on the Orient Express / Agatha Christie’ (F32) materialized the publication ‘Murder on the Orient Express / Agatha Christie’ published by HarperCollins 2017 (F3).
- The printing of the score of Bach’s ‘Goldberg Variations’ by Balthasar Schmid in 1741 (F32) materialized the publication Bach’s ‘Goldberg Variations’ as published by Balthasar Schmid in 1741 (F3).
</rdfs:comment>
  </owl:ObjectProperty>
  <owl:ObjectProperty rdf:about="R27i_was_materialized_by">
    <rdfs:label xml:lang="en">R27i was materialized by</rdfs:label>
    <skos:notation>R27i</skos:notation>
    <skos:prefLabel xml:lang="en">was materialized by</skos:prefLabel>
    <rdfs:domain rdf:resource="http://iflastandards.info/ns/lrm/lrmoo/F3_Manifestation"/>
    <rdfs:range rdf:resource="http://iflastandards.info/ns/lrm/lrmoo/F32_Item_Production_Event"/>
    <owl:inverseOf rdf:resource="http://iflastandards.info/ns/lrm/lrmoo/R27_materialized"/>
    <rdfs:subPropertyOf rdf:resource="http://www.cidoc-crm.org/cidoc-crm/P16i_was_used_for"/>
    <rdfs:comment xml:lang="en">Quantification of the inverse property: many to many (0,n:0,n)

Scope note of the inverse property:
This property associates an instance of F32 Item Production Event with the set of signs provided by the publisher to be carried by all of the produced items (i.e., the instances of F5 Item) and any other physical features foreseen as integral to the instance of F3 Manifestation that is materialised.

Examples of the inverse property:
- The production of copies of the paperback edition of the HarperCollins 2017 publication ‘Murder on the Orient Express / Agatha Christie’ (F32) materialized the publication ‘Murder on the Orient Express / Agatha Christie’ published by HarperCollins 2017 (F3).
- The printing of the score of Bach’s ‘Goldberg Variations’ by Balthasar Schmid in 1741 (F32) materialized the publication Bach’s ‘Goldberg Variations’ as published by Balthasar Schmid in 1741 (F3).
</rdfs:comment>
  </owl:ObjectProperty>
  <owl:ObjectProperty rdf:about="R28_produced">
    <rdfs:label xml:lang="en">R28 produced</rdfs:label>
    <skos:notation>R28</skos:notation>
    <skos:prefLabel xml:lang="en">produced</skos:prefLabel>
    <rdfs:domain rdf:resource="http://iflastandards.info/ns/lrm/lrmoo/F32_Item_Production_Event"/>
    <rdfs:range rdf:resource="http://iflastandards.info/ns/lrm/lrmoo/F5_Item"/>
    <owl:inverseOf rdf:resource="http://iflastandards.info/ns/lrm/lrmoo/R28i_was_produced_by"/>
    <rdfs:subPropertyOf rdf:resource="http://www.cidoc-crm.org/cidoc-crm/P108_has_produced"/>
    <rdfs:comment xml:lang="en">Quantification: one to many, necessary, dependent (1,n:1,1)

Scope note:
This property associates an instance of F32 Item Production Event with any one of the produced items (i.e., the instances of F5 Item).

Examples:
- The production of copies of the paperback edition of the HarperCollins 2017 publication ‘Murder on the Orient Express / Agatha Christie’ (F32) produced the copy (item) of this publication that is held by the Deichman public library in Oslo, Norway, and which is identified by inventory number ‘9138513’ (F5).
- The printing of the score of Bach’s ‘Goldberg Variations’ by Balthasar Schmid in 1741 (F32) produced the copy of this score (item) that is held by the National Library in France (F5).
- The second print run, occurring in 1978, of the publication dated of 1972 and entitled ‘The complete poems of Stephen Crane, edited with an introduction by Joseph Katz’ (identified by ISBN ‘0-8014-9130-4’) (F32) produced Universitätsbibliothek Passau’s holding identified by call number ‘00/HT 4801.978 K2’ (F5).
</rdfs:comment>
  </owl:ObjectProperty>
  <owl:ObjectProperty rdf:about="R28i_was_produced_by">
    <rdfs:label xml:lang="en">R28i was produced by</rdfs:label>
    <skos:notation>R28i</skos:notation>
    <skos:prefLabel xml:lang="en">was produced by</skos:prefLabel>
    <rdfs:domain rdf:resource="http://iflastandards.info/ns/lrm/lrmoo/F5_Item"/>
    <rdfs:range rdf:resource="http://iflastandards.info/ns/lrm/lrmoo/F32_Item_Production_Event"/>
    <owl:inverseOf rdf:resource="http://iflastandards.info/ns/lrm/lrmoo/R28_produced"/>
    <rdfs:subPropertyOf rdf:resource="http://www.cidoc-crm.org/cidoc-crm/P108i_was_produced_by"/>
    <rdfs:comment xml:lang="en">Quantification of the inverse property: one to many, necessary, dependent (1,n:1,1)

Scope note of the inverse property:
This property associates an instance of F32 Item Production Event with any one of the produced items (i.e., the instances of F5 Item).

Examples of the inverse property:
- The production of copies of the paperback edition of the HarperCollins 2017 publication ‘Murder on the Orient Express / Agatha Christie’ (F32) produced the copy (item) of this publication that is held by the Deichman public library in Oslo, Norway, and which is identified by inventory number ‘9138513’ (F5).
- The printing of the score of Bach’s ‘Goldberg Variations’ by Balthasar Schmid in 1741 (F32) produced the copy of this score (item) that is held by the National Library in France (F5).
- The second print run, occurring in 1978, of the publication dated of 1972 and entitled ‘The complete poems of Stephen Crane, edited with an introduction by Joseph Katz’ (identified by ISBN ‘0-8014-9130-4’) (F32) produced Universitätsbibliothek Passau’s holding identified by call number ‘00/HT 4801.978 K2’ (F5).
</rdfs:comment>
  </owl:ObjectProperty>
  <owl:ObjectProperty rdf:about="R29_reproduced_object">
    <rdfs:label xml:lang="en">R29 reproduced object</rdfs:label>
    <skos:notation>R29</skos:notation>
    <skos:prefLabel xml:lang="en">reproduced object</skos:prefLabel>
    <rdfs:domain rdf:resource="http://iflastandards.info/ns/lrm/lrmoo/F33_Reproduction_Event"/>
    <rdfs:range rdf:resource="http://iflastandards.info/ns/lrm/lrmoo/F5_Item"/>
    <owl:inverseOf rdf:resource="http://iflastandards.info/ns/lrm/lrmoo/R29i_was_object_reproduced_by"/>
    <rdfs:subPropertyOf rdf:resource="http://www.cidoc-crm.org/cidoc-crm/P16_used_specific_object"/>
    <rdfs:comment xml:lang="en">Quantification: many to many, necessary (1,n:0,n)

Scope note:
This property associates an instance of F33 Reproduction Event with an instance of F5 Item it reproduces.

Examples:
- The activity performed by Schott when producing the 2015 publication of Harry Partch’s ‘Two studies on ancient Greek scales’ (F33) reproduced object Harry Partch’s holograph manuscript of ‘Two studies on ancient Greek scales’ (F5).
</rdfs:comment>
  </owl:ObjectProperty>
  <owl:ObjectProperty rdf:about="R29i_was_object_reproduced_by">
    <rdfs:label xml:lang="en">R29i was object reproduced by</rdfs:label>
    <skos:notation>R29i</skos:notation>
    <skos:prefLabel xml:lang="en">was object reproduced by</skos:prefLabel>
    <rdfs:domain rdf:resource="http://iflastandards.info/ns/lrm/lrmoo/F5_Item"/>
    <rdfs:range rdf:resource="http://iflastandards.info/ns/lrm/lrmoo/F33_Reproduction_Event"/>
    <owl:inverseOf rdf:resource="http://iflastandards.info/ns/lrm/lrmoo/R29_reproduced_object"/>
    <rdfs:subPropertyOf rdf:resource="http://www.cidoc-crm.org/cidoc-crm/P16i_was_used_for"/>
    <rdfs:comment xml:lang="en">Quantification of the inverse property: many to many, necessary (1,n:0,n)

Scope note of the inverse property:
This property associates an instance of F33 Reproduction Event with an instance of F5 Item it reproduces.

Examples of the inverse property:
- The activity performed by Schott when producing the 2015 publication of Harry Partch’s ‘Two studies on ancient Greek scales’ (F33) reproduced object Harry Partch’s holograph manuscript of ‘Two studies on ancient Greek scales’ (F5).
</rdfs:comment>
  </owl:ObjectProperty>
  <owl:ObjectProperty rdf:about="R30_reproduced_publication">
    <rdfs:label xml:lang="en">R30 reproduced publication</rdfs:label>
    <skos:notation>R30</skos:notation>
    <skos:prefLabel xml:lang="en">reproduced publication</skos:prefLabel>
    <rdfs:domain rdf:resource="http://iflastandards.info/ns/lrm/lrmoo/F33_Reproduction_Event"/>
    <rdfs:range rdf:resource="http://iflastandards.info/ns/lrm/lrmoo/F3_Manifestation"/>
    <owl:inverseOf rdf:resource="http://iflastandards.info/ns/lrm/lrmoo/R30i_was_publication_reproduced_by"/>
    <rdfs:subPropertyOf rdf:resource="http://www.cidoc-crm.org/cidoc-crm/P16_used_specific_object"/>
    <rdfs:comment xml:lang="en">Quantification: many to many, necessary (1,n:0,n)

Scope note:
This property associates an instance of F33 Reproduction Event with an instance of F3 Manifestation it reproduces.

Examples:
- The activity performed by Cambridge University Press when producing the 2014 publication of Daniel Wilson’s ‘Caliban: the missing link’ (F33) reproduced publication the 1873 publication of Daniel Wilson’s ‘Caliban: the missing link’ by Macmillan (F3).
- The activity performed by the Éditions du Seuil when producing the 2007 publication of Hubert Reeve’s ‘Malicorne: réflexions d’un observateur de la nature’ as number 179 in the series ‘Points. Science’ (identified by ISBN ‘978-2-02-096760-0’) (F33) reproduced publication the 1990 publication by the Éditions du Seuil in the series ‘Science ouverte’ (identified by ISBN ‘2-02-012644-3’) (F3).
</rdfs:comment>
  </owl:ObjectProperty>
  <owl:ObjectProperty rdf:about="R30i_was_publication_reproduced_by">
    <rdfs:label xml:lang="en">R30i was publication reproduced by</rdfs:label>
    <skos:notation>R30i</skos:notation>
    <skos:prefLabel xml:lang="en">was publication reproduced by</skos:prefLabel>
    <rdfs:domain rdf:resource="http://iflastandards.info/ns/lrm/lrmoo/F3_Manifestation"/>
    <rdfs:range rdf:resource="http://iflastandards.info/ns/lrm/lrmoo/F33_Reproduction_Event"/>
    <owl:inverseOf rdf:resource="http://iflastandards.info/ns/lrm/lrmoo/R30_reproduced_publication"/>
    <rdfs:subPropertyOf rdf:resource="http://www.cidoc-crm.org/cidoc-crm/P16i_was_used_for"/>
    <rdfs:comment xml:lang="en">Quantification of the inverse property: many to many, necessary (1,n:0,n)

Scope note of the inverse property:
This property associates an instance of F33 Reproduction Event with an instance of F3 Manifestation it reproduces.

Examples of the inverse property:
- The activity performed by Cambridge University Press when producing the 2014 publication of Daniel Wilson’s ‘Caliban: the missing link’ (F33) reproduced publication the 1873 publication of Daniel Wilson’s ‘Caliban: the missing link’ by Macmillan (F3).
- The activity performed by the Éditions du Seuil when producing the 2007 publication of Hubert Reeve’s ‘Malicorne: réflexions d’un observateur de la nature’ as number 179 in the series ‘Points. Science’ (identified by ISBN ‘978-2-02-096760-0’) (F33) reproduced publication the 1990 publication by the Éditions du Seuil in the series ‘Science ouverte’ (identified by ISBN ‘2-02-012644-3’) (F3).
</rdfs:comment>
  </owl:ObjectProperty>
  <owl:DatatypeProperty rdf:about="R33_has_string">
    <rdfs:label xml:lang="en">R33 has string</rdfs:label>
    <skos:notation>R33</skos:notation>
    <skos:prefLabel xml:lang="en">has string</skos:prefLabel>
    <rdfs:domain rdf:resource="http://iflastandards.info/ns/lrm/lrmoo/F12_Nomen"/>
    <rdfs:subPropertyOf rdf:resource="http://www.cidoc-crm.org/cidoc-crm/P3_has_note"/>
    <rdfs:comment xml:lang="en">Quantification: many to one, necessary (1,1:0,n)

Scope note:
This property associates an instance of F12 Nomen with a sign or arrangement of signs that is used to refer to something through that instance of F12 Nomen.

Examples:
- The English word ‘poison’ as a term for toxic substances, in written form in the Latin alphabet (F12) has string the letters p, o, i, s, o, n with no intervening spaces (E62).
- The English word ‘poison’ as a term for toxic substances, notated in the International Phonetic Alphabet (F12) has string the string of characters ['pɔɪz(ə)n] (E62).
- The French word ‘poison’ as a term for toxic substances, in written form in the Latin alphabet (F12) has string the letters p, o, i, s, o, n with no intervening spaces (E62).
- The French word ‘poison’ as a term for toxic substances, notated in the International Phonetic Alphabet (F12) has string the string of characters [pwa'zɔ̃] (E62).
</rdfs:comment>
  </owl:DatatypeProperty>
  <owl:ObjectProperty rdf:about="R35_is_specified_by">
    <rdfs:label xml:lang="en">R35 is specified by</rdfs:label>
    <skos:notation>R35</skos:notation>
    <skos:prefLabel xml:lang="en">is specified by</skos:prefLabel>
    <rdfs:domain rdf:resource="http://iflastandards.info/ns/lrm/lrmoo/F12_Nomen"/>
    <rdfs:range rdf:resource="http://iflastandards.info/ns/lrm/lrmoo/F2_Expression"/>
    <owl:inverseOf rdf:resource="http://iflastandards.info/ns/lrm/lrmoo/R35i_specifies"/>
    <rdfs:subPropertyOf rdf:resource="http://www.cidoc-crm.org/cidoc-crm/P67i_is_referred_to_by"/>
    <rdfs:comment xml:lang="en">Quantification: many to one, necessary, dependent (1,1:1,n)

Scope note:
This property associates an instance of F12 Nomen with an instance of F2 Expression which documents, defines or provides evidence for the particular nomen in the stated sense.

Examples:
- ‘acoustic surface wave device’ as a term for the device (F12) is specified by INSPEC Thesaurus version January 1973 (F2).
- ‘595.7’ as a classification number for the taxonomic class Insecta (insects) (F12) is specified by the 23(rd) edition of the Dewey Decimal Classification (DDC) (F2).
- ‘Martin Doerr’ as the name of a co-chair of the CIDOC CRM SIG (F12) is specified by the statement on the title page of the Definition of the ‘CIDOC Conceptual Reference Model’, Version 7.1.3, February 2024 (F2).
</rdfs:comment>
  </owl:ObjectProperty>
  <owl:ObjectProperty rdf:about="R35i_specifies">
    <rdfs:label xml:lang="en">R35i specifies</rdfs:label>
    <skos:notation>R35i</skos:notation>
    <skos:prefLabel xml:lang="en">specifies</skos:prefLabel>
    <rdfs:domain rdf:resource="http://iflastandards.info/ns/lrm/lrmoo/F2_Expression"/>
    <rdfs:range rdf:resource="http://iflastandards.info/ns/lrm/lrmoo/F12_Nomen"/>
    <owl:inverseOf rdf:resource="http://iflastandards.info/ns/lrm/lrmoo/R35_is_specified_by"/>
    <rdfs:subPropertyOf rdf:resource="http://www.cidoc-crm.org/cidoc-crm/P67_refers_to"/>
    <rdfs:comment xml:lang="en">Quantification of the inverse property: many to one, necessary, dependent (1,1:1,n)

Scope note of the inverse property:
This property associates an instance of F12 Nomen with an instance of F2 Expression which documents, defines or provides evidence for the particular nomen in the stated sense.

Examples of the inverse property:
- ‘acoustic surface wave device’ as a term for the device (F12) is specified by INSPEC Thesaurus version January 1973 (F2).
- ‘595.7’ as a classification number for the taxonomic class Insecta (insects) (F12) is specified by the 23(rd) edition of the Dewey Decimal Classification (DDC) (F2).
- ‘Martin Doerr’ as the name of a co-chair of the CIDOC CRM SIG (F12) is specified by the statement on the title page of the Definition of the ‘CIDOC Conceptual Reference Model’, Version 7.1.3, February 2024 (F2).
</rdfs:comment>
  </owl:ObjectProperty>
  <owl:ObjectProperty rdf:about="R36_uses_script_conversion">
    <rdfs:label xml:lang="en">R36 uses script conversion</rdfs:label>
    <skos:notation>R36</skos:notation>
    <skos:prefLabel xml:lang="en">uses script conversion</skos:prefLabel>
    <rdfs:domain rdf:resource="http://iflastandards.info/ns/lrm/lrmoo/F12_Nomen"/>
    <rdfs:range rdf:resource="http://iflastandards.info/ns/lrm/lrmoo/F36_Script_Conversion"/>
    <owl:inverseOf rdf:resource="http://iflastandards.info/ns/lrm/lrmoo/R36i_is_script_conversion_used_in"/>
    <rdfs:comment xml:lang="en">Quantification: many to many (0,n:0,n)

Shortcut Of: F12 Nomen. R17i was created by (created): E65 Creation. P33 used specific technique (was used by): E29 Design or Procedure

Scope note:
This property associates an instance of F12 Nomen with an instance of F36 Script Conversion that is used to create the E62 String used in that instance of F12 Nomen from the string used in another instance of F12 Nomen that co-refers with the first nomen (the instances of F12 Nomen are related via the R56 has related form (is related form of) property). The source of this conversion may or may not be explicitly mentioned.

Examples:
- ‘Du Fu’ as the name for a Chinese poet of the 8(th) century (F12) uses script conversion Pinyin (F36).
- ‘Čajkovskij, Petr Ilʹič’ as the name of a Russian composer (F12) uses script conversion ‘ISO 9:1995 Information and documentation — Transliteration of Cyrillic characters into Latin characters — Slavic and non-Slavic languages’ (F36).
</rdfs:comment>
  </owl:ObjectProperty>
  <owl:ObjectProperty rdf:about="R36i_is_script_conversion_used_in">
    <rdfs:label xml:lang="en">R36i is script conversion used in</rdfs:label>
    <skos:notation>R36i</skos:notation>
    <skos:prefLabel xml:lang="en">is script conversion used in</skos:prefLabel>
    <rdfs:domain rdf:resource="http://iflastandards.info/ns/lrm/lrmoo/F36_Script_Conversion"/>
    <rdfs:range rdf:resource="http://iflastandards.info/ns/lrm/lrmoo/F12_Nomen"/>
    <owl:inverseOf rdf:resource="http://iflastandards.info/ns/lrm/lrmoo/R36_uses_script_conversion"/>
    <rdfs:comment xml:lang="en">Quantification of the inverse property: many to many (0,n:0,n)

Shortcut Of of the inverse property: F12 Nomen. R17i was created by (created): E65 Creation. P33 used specific technique (was used by): E29 Design or Procedure

Scope note of the inverse property:
This property associates an instance of F12 Nomen with an instance of F36 Script Conversion that is used to create the E62 String used in that instance of F12 Nomen from the string used in another instance of F12 Nomen that co-refers with the first nomen (the instances of F12 Nomen are related via the R56 has related form (is related form of) property). The source of this conversion may or may not be explicitly mentioned.

Examples of the inverse property:
- ‘Du Fu’ as the name for a Chinese poet of the 8(th) century (F12) uses script conversion Pinyin (F36).
- ‘Čajkovskij, Petr Ilʹič’ as the name of a Russian composer (F12) uses script conversion ‘ISO 9:1995 Information and documentation — Transliteration of Cyrillic characters into Latin characters — Slavic and non-Slavic languages’ (F36).
</rdfs:comment>
  </owl:ObjectProperty>
  <owl:ObjectProperty rdf:about="R54_has_language">
    <rdfs:label xml:lang="en">R54 has language</rdfs:label>
    <skos:notation>R54</skos:notation>
    <skos:prefLabel xml:lang="en">has language</skos:prefLabel>
    <rdfs:domain rdf:resource="http://iflastandards.info/ns/lrm/lrmoo/F12_Nomen"/>
    <rdfs:range rdf:resource="http://www.cidoc-crm.org/cidoc-crm/E56_Language"/>
    <owl:inverseOf rdf:resource="http://iflastandards.info/ns/lrm/lrmoo/R54i_is_language_of"/>
    <rdfs:subPropertyOf rdf:resource="http://www.cidoc-crm.org/cidoc-crm/P2_has_type"/>
    <rdfs:comment xml:lang="en">Quantification: many to many (0,n:0,n)

Scope note:
This property associates an instance of F12 Nomen with an instance of E56 Language which is the language used for or associated with the nomen.

Examples:
- ‘Colón Cristóbal’ as a name of the explorer and navigator (F12) has language Spanish [encoded as ‘spa’ in set 2 of ISO 639:2023] (E56).
- ‘Columbus Christopher’ as a name of the explorer and navigator (F12) has language English [encoded as ‘eng’ in set 2 of ISO 639:2023] (E56).
- ‘Conseil international des musées’ as a name of ICOM, the International Council of Museums (F12) has language French [encoded as ‘fre’ in set 2 of ISO 639:2023] (E56).
- ‘Internationaler Museumsrat’ as a name of ICOM, the International Council of Museums (F12) has language German [encoded as ‘ger’ in set 2 of ISO 639:2023] (E56).
- ‘Union européenne’ as a name of the European Union (F12) has language French [encoded as ‘fre’ in set 2 of ISO 639:2023] (E56).
- ‘Vienna’ as a name of the city which is the capital of Austria (F12) has language English [encoded as ‘eng’ in set 2 of ISO 639:2023] (E56).
- ‘Organic chemistry’ as a term for the branch of chemistry concerned with organic compounds (F12) has language English [encoded as ‘eng’ in set 2 of ISO 639:2023] (E56).
</rdfs:comment>
  </owl:ObjectProperty>
  <owl:ObjectProperty rdf:about="R54i_is_language_of">
    <rdfs:label xml:lang="en">R54i is language of</rdfs:label>
    <skos:notation>R54i</skos:notation>
    <skos:prefLabel xml:lang="en">is language of</skos:prefLabel>
    <rdfs:domain rdf:resource="http://www.cidoc-crm.org/cidoc-crm/E56_Language"/>
    <rdfs:range rdf:resource="http://iflastandards.info/ns/lrm/lrmoo/F12_Nomen"/>
    <owl:inverseOf rdf:resource="http://iflastandards.info/ns/lrm/lrmoo/R54_has_language"/>
    <rdfs:subPropertyOf rdf:resource="http://www.cidoc-crm.org/cidoc-crm/P2i_is_type_of"/>
    <rdfs:comment xml:lang="en">Quantification of the inverse property: many to many (0,n:0,n)

Scope note of the inverse property:
This property associates an instance of F12 Nomen with an instance of E56 Language which is the language used for or associated with the nomen.

Examples of the inverse property:
- ‘Colón Cristóbal’ as a name of the explorer and navigator (F12) has language Spanish [encoded as ‘spa’ in set 2 of ISO 639:2023] (E56).
- ‘Columbus Christopher’ as a name of the explorer and navigator (F12) has language English [encoded as ‘eng’ in set 2 of ISO 639:2023] (E56).
- ‘Conseil international des musées’ as a name of ICOM, the International Council of Museums (F12) has language French [encoded as ‘fre’ in set 2 of ISO 639:2023] (E56).
- ‘Internationaler Museumsrat’ as a name of ICOM, the International Council of Museums (F12) has language German [encoded as ‘ger’ in set 2 of ISO 639:2023] (E56).
- ‘Union européenne’ as a name of the European Union (F12) has language French [encoded as ‘fre’ in set 2 of ISO 639:2023] (E56).
- ‘Vienna’ as a name of the city which is the capital of Austria (F12) has language English [encoded as ‘eng’ in set 2 of ISO 639:2023] (E56).
- ‘Organic chemistry’ as a term for the branch of chemistry concerned with organic compounds (F12) has language English [encoded as ‘eng’ in set 2 of ISO 639:2023] (E56).
</rdfs:comment>
  </owl:ObjectProperty>
  <owl:ObjectProperty rdf:about="R56_has_related_form">
    <rdfs:label xml:lang="en">R56 has related form</rdfs:label>
    <skos:notation>R56</skos:notation>
    <skos:prefLabel xml:lang="en">has related form</skos:prefLabel>
    <rdfs:domain rdf:resource="http://iflastandards.info/ns/lrm/lrmoo/F12_Nomen"/>
    <rdfs:range rdf:resource="http://iflastandards.info/ns/lrm/lrmoo/F12_Nomen"/>
    <owl:inverseOf rdf:resource="http://iflastandards.info/ns/lrm/lrmoo/R56i_is_related_form_of"/>
    <rdfs:comment xml:lang="en">Quantification: many to many (0,n:0,n)

Shortcut Of: E89 Propositional Object (1). P67 refers to: E1 CRM Entity. P67i is referred to by: E89 Propositional Object (2)

Scope note:
This property associates an instance of F12 Nomen with another instance of F12 Nomen which co-refers to the same instance of E1 CRM Entity. This property is not transitive. It is symmetric and irreflexive.

Examples:
- ‘Čajkovskij, Petr Ilʹič’ as the name of the Russian composer (F12) has related form ‘Пётр Ильич Чайковский’ as the name of the Russian composer (F12) with has type Transliteration (E55).
- ‘The Lord of the Rings’ as the title of the work by J. R. R. Tolkien (F12) has related form ‘Le Seigneur des anneaux’ as the title of the work by J. R. R. Tolkien (F12) with has type Original language (E55).
- ‘IFLA’ as the name of the international association in the library field (F12) has related form ‘International Federation of Library Associations and Institutions’ as the name of the international association in the library field (F12) with has type Acronym (E55).
- ‘Siam’ as the name of the country in South Asia (F12) has related form ‘Thailand’ as the name of the country in South Asia (F12).
- ‘595.7’ as a classification number referring to the taxonomic class insects (F12) has related form ‘Insecta’ as a term referring to the taxonomic class insects (F12). [The latter being the caption for the Dewey Decimal Classification number in the English language 23(rd) edition.]

Properties:
- R56.1 has type: 
  Scope note:
    This property allows for specifying the particular kind of relationship that holds between the domain nomen and the range nomen, such as by being a derivation, an alternative, a lexical variant, etc. Typing the association may cause loss of symmetry.
</rdfs:comment>
  </owl:ObjectProperty>
  <owl:ObjectProperty rdf:about="R56i_is_related_form_of">
    <rdfs:label xml:lang="en">R56i is related form of</rdfs:label>
    <skos:notation>R56i</skos:notation>
    <skos:prefLabel xml:lang="en">is related form of</skos:prefLabel>
    <rdfs:domain rdf:resource="http://iflastandards.info/ns/lrm/lrmoo/F12_Nomen"/>
    <rdfs:range rdf:resource="http://iflastandards.info/ns/lrm/lrmoo/F12_Nomen"/>
    <owl:inverseOf rdf:resource="http://iflastandards.info/ns/lrm/lrmoo/R56_has_related_form"/>
    <rdfs:comment xml:lang="en">Quantification of the inverse property: many to many (0,n:0,n)

Shortcut Of of the inverse property: E89 Propositional Object (1). P67 refers to: E1 CRM Entity. P67i is referred to by: E89 Propositional Object (2)

Scope note of the inverse property:
This property associates an instance of F12 Nomen with another instance of F12 Nomen which co-refers to the same instance of E1 CRM Entity. This property is not transitive. It is symmetric and irreflexive.

Examples of the inverse property:
- ‘Čajkovskij, Petr Ilʹič’ as the name of the Russian composer (F12) has related form ‘Пётр Ильич Чайковский’ as the name of the Russian composer (F12) with has type Transliteration (E55).
- ‘The Lord of the Rings’ as the title of the work by J. R. R. Tolkien (F12) has related form ‘Le Seigneur des anneaux’ as the title of the work by J. R. R. Tolkien (F12) with has type Original language (E55).
- ‘IFLA’ as the name of the international association in the library field (F12) has related form ‘International Federation of Library Associations and Institutions’ as the name of the international association in the library field (F12) with has type Acronym (E55).
- ‘Siam’ as the name of the country in South Asia (F12) has related form ‘Thailand’ as the name of the country in South Asia (F12).
- ‘595.7’ as a classification number referring to the taxonomic class insects (F12) has related form ‘Insecta’ as a term referring to the taxonomic class insects (F12). [The latter being the caption for the Dewey Decimal Classification number in the English language 23(rd) edition.]
</rdfs:comment>
  </owl:ObjectProperty>
  <owl:ObjectProperty rdf:about="R67_has_part">
    <rdfs:label xml:lang="en">R67 has part</rdfs:label>
    <skos:notation>R67</skos:notation>
    <skos:prefLabel xml:lang="en">has part</skos:prefLabel>
    <rdfs:domain rdf:resource="http://iflastandards.info/ns/lrm/lrmoo/F1_Work"/>
    <rdfs:range rdf:resource="http://iflastandards.info/ns/lrm/lrmoo/F1_Work"/>
    <owl:inverseOf rdf:resource="http://iflastandards.info/ns/lrm/lrmoo/R67i_forms_part_of"/>
    <rdfs:subPropertyOf rdf:resource="http://www.cidoc-crm.org/cidoc-crm/P148_has_component"/>
    <rdfs:comment xml:lang="en">Quantification: many to many (0,n:0,n)

Scope note:
This property associates an instance of F1 Work with another instance of F1 Work that forms part of it in a complementary role to other sibling parts, conceived at some point in time to form together a logical whole, such as the parts of a trilogy. This property is transitive, asymmetric and irreflexive.

Examples:
- Ursula K. Le Guin’s textual work ‘The Earthsea trilogy’ (F1) has part Ursula K. Le Guin’s textual work ‘The tombs of Atuan’ (F1).
- Dante Alighieri’s textual work entitled ‘Divina Commedia’ (F1) has part Dante Alighieri’s textual work entitled ‘Inferno’ (F1).
- Miguel de Cervantes’ textual work entitled ‘Don Quixote’ (F1) has part Miguel de Cervantes’ textual work entitled ‘El ingenioso hidalgo Don Quixote de la Mancha’ (F1).
- Miguel de Cervantes’ textual work entitled ‘Don Quixote’ (F1) has part Miguel de Cervantes’ textual work entitled ‘Segunda Parte del Ingenioso Cavallero Don Quixote de la Mancha’ (F1).
- J. R. R. Tolkien’s textual work ‘The Lord of the Rings’ (F1) has part J. R. R. Tolkien’s textual work ‘The Two Towers’ (F1).
- Cormac McCarthy’s textual work ‘The Border Trilogy’ (F1) has part Cormac McCarthy’s textual work ‘All the Pretty Horses’ (F1).
- Giovanni Battista Piranesi’s graphic work entitled ‘Carceri’ (F1) has part Giovanni Battista Piranesi’s graphic work entitled ‘Carcere XVI: the pier with chains’ (F1).
- Ludwig van Beethoven’s musical work entitled ‘Symphony No. 9’ (F1) has part Ludwig van Beethoven’s musical work ‘Finale’ (4(th) movement) (F1).
- Johann Sebastian Bach’s musical work ‘Goldberg Variations’ (F1) has part the musical work entitled ‘Variatio 1. a 1 Clav’ (F1).
</rdfs:comment>
  </owl:ObjectProperty>
  <owl:ObjectProperty rdf:about="R67i_forms_part_of">
    <rdfs:label xml:lang="en">R67i forms part of</rdfs:label>
    <skos:notation>R67i</skos:notation>
    <skos:prefLabel xml:lang="en">forms part of</skos:prefLabel>
    <rdfs:domain rdf:resource="http://iflastandards.info/ns/lrm/lrmoo/F1_Work"/>
    <rdfs:range rdf:resource="http://iflastandards.info/ns/lrm/lrmoo/F1_Work"/>
    <owl:inverseOf rdf:resource="http://iflastandards.info/ns/lrm/lrmoo/R67_has_part"/>
    <rdfs:subPropertyOf rdf:resource="http://www.cidoc-crm.org/cidoc-crm/P148i_is_component_of"/>
    <rdfs:comment xml:lang="en">Quantification of the inverse property: many to many (0,n:0,n)

Scope note of the inverse property:
This property associates an instance of F1 Work with another instance of F1 Work that forms part of it in a complementary role to other sibling parts, conceived at some point in time to form together a logical whole, such as the parts of a trilogy. This property is transitive, asymmetric and irreflexive.

Examples of the inverse property:
- Ursula K. Le Guin’s textual work ‘The Earthsea trilogy’ (F1) has part Ursula K. Le Guin’s textual work ‘The tombs of Atuan’ (F1).
- Dante Alighieri’s textual work entitled ‘Divina Commedia’ (F1) has part Dante Alighieri’s textual work entitled ‘Inferno’ (F1).
- Miguel de Cervantes’ textual work entitled ‘Don Quixote’ (F1) has part Miguel de Cervantes’ textual work entitled ‘El ingenioso hidalgo Don Quixote de la Mancha’ (F1).
- Miguel de Cervantes’ textual work entitled ‘Don Quixote’ (F1) has part Miguel de Cervantes’ textual work entitled ‘Segunda Parte del Ingenioso Cavallero Don Quixote de la Mancha’ (F1).
- J. R. R. Tolkien’s textual work ‘The Lord of the Rings’ (F1) has part J. R. R. Tolkien’s textual work ‘The Two Towers’ (F1).
- Cormac McCarthy’s textual work ‘The Border Trilogy’ (F1) has part Cormac McCarthy’s textual work ‘All the Pretty Horses’ (F1).
- Giovanni Battista Piranesi’s graphic work entitled ‘Carceri’ (F1) has part Giovanni Battista Piranesi’s graphic work entitled ‘Carcere XVI: the pier with chains’ (F1).
- Ludwig van Beethoven’s musical work entitled ‘Symphony No. 9’ (F1) has part Ludwig van Beethoven’s musical work ‘Finale’ (4(th) movement) (F1).
- Johann Sebastian Bach’s musical work ‘Goldberg Variations’ (F1) has part the musical work entitled ‘Variatio 1. a 1 Clav’ (F1).
</rdfs:comment>
  </owl:ObjectProperty>
  <owl:ObjectProperty rdf:about="R68_is_inspired_by">
    <rdfs:label xml:lang="en">R68 is inspired by</rdfs:label>
    <skos:notation>R68</skos:notation>
    <skos:prefLabel xml:lang="en">is inspired by</skos:prefLabel>
    <rdfs:domain rdf:resource="http://iflastandards.info/ns/lrm/lrmoo/F1_Work"/>
    <rdfs:range rdf:resource="http://iflastandards.info/ns/lrm/lrmoo/F1_Work"/>
    <owl:inverseOf rdf:resource="http://iflastandards.info/ns/lrm/lrmoo/R68i_is_inspiration_for"/>
    <rdfs:subPropertyOf rdf:resource="http://www.cidoc-crm.org/cidoc-crm/P130_shows_features_of"/>
    <rdfs:comment xml:lang="en">Quantification: many to many (0,n:0,n)

Shortcut Of: F1 Work (2). R16i was created by: F27 Work Creation. P15 was influenced by: F1 Work (1)

Scope note:
This property associates an instance of F1 Work with another instance of F1 Work whose content was inspired by that instance of F1 Work. The content of the range work instance served in some way as a source of ideas for the domain work instance. Neither instance of F1 Work may be a part of the other. This property is not transitive. It is irreflexive.

Examples:
- The musical ‘West Side Story’ (F1) is inspired by the play ‘Romeo and Juliet’ by William Shakespeare (F1).
- The play ‘Rosencrantz and Guildenstern are Dead’ by Tom Stoppard (F1) is inspired by the play ‘The Tragedy of Hamlet, Prince of Denmark’ by William Shakespeare (F1).
- The musical work ‘The Great Gate of Kiev’ (F1) from ‘Pictures at an Exhibition’ by Modest Mussorgsky is inspired by the painting ‘Plan for a City Gate in Kiev’ by Viktor Hartmann (F1).
- The board game ‘War of the Ring’ by Roberto Di Meglio, Marco Maggi and Francesco Nepitello (F1) is inspired by the literary work ‘The Lord of the Rings’ by J. R. R. Tolkien (F1).
- The literary work ‘Girl with a Pearl Earring’ by Tracy Chevalier (F1) is inspired by the painting ‘Girl with a Pearl Earring’ by Johannes Vermeer (F1).
</rdfs:comment>
  </owl:ObjectProperty>
  <owl:ObjectProperty rdf:about="R68i_is_inspiration_for">
    <rdfs:label xml:lang="en">R68i is inspiration for</rdfs:label>
    <skos:notation>R68i</skos:notation>
    <skos:prefLabel xml:lang="en">is inspiration for</skos:prefLabel>
    <rdfs:domain rdf:resource="http://iflastandards.info/ns/lrm/lrmoo/F1_Work"/>
    <rdfs:range rdf:resource="http://iflastandards.info/ns/lrm/lrmoo/F1_Work"/>
    <owl:inverseOf rdf:resource="http://iflastandards.info/ns/lrm/lrmoo/R68_is_inspired_by"/>
    <rdfs:subPropertyOf rdf:resource="http://www.cidoc-crm.org/cidoc-crm/P130i_features_are_also_found_on"/>
    <rdfs:comment xml:lang="en">Quantification of the inverse property: many to many (0,n:0,n)

Shortcut Of of the inverse property: F1 Work (2). R16i was created by: F27 Work Creation. P15 was influenced by: F1 Work (1)

Scope note of the inverse property:
This property associates an instance of F1 Work with another instance of F1 Work whose content was inspired by that instance of F1 Work. The content of the range work instance served in some way as a source of ideas for the domain work instance. Neither instance of F1 Work may be a part of the other. This property is not transitive. It is irreflexive.

Examples of the inverse property:
- The musical ‘West Side Story’ (F1) is inspired by the play ‘Romeo and Juliet’ by William Shakespeare (F1).
- The play ‘Rosencrantz and Guildenstern are Dead’ by Tom Stoppard (F1) is inspired by the play ‘The Tragedy of Hamlet, Prince of Denmark’ by William Shakespeare (F1).
- The musical work ‘The Great Gate of Kiev’ (F1) from ‘Pictures at an Exhibition’ by Modest Mussorgsky is inspired by the painting ‘Plan for a City Gate in Kiev’ by Viktor Hartmann (F1).
- The board game ‘War of the Ring’ by Roberto Di Meglio, Marco Maggi and Francesco Nepitello (F1) is inspired by the literary work ‘The Lord of the Rings’ by J. R. R. Tolkien (F1).
- The literary work ‘Girl with a Pearl Earring’ by Tracy Chevalier (F1) is inspired by the painting ‘Girl with a Pearl Earring’ by Johannes Vermeer (F1).
</rdfs:comment>
  </owl:ObjectProperty>
  <owl:ObjectProperty rdf:about="R69_has_physical_form">
    <rdfs:label xml:lang="en">R69 has physical form</rdfs:label>
    <skos:notation>R69</skos:notation>
    <skos:prefLabel xml:lang="en">has physical form</skos:prefLabel>
    <rdfs:domain rdf:resource="http://iflastandards.info/ns/lrm/lrmoo/F3_Manifestation"/>
    <rdfs:range rdf:resource="http://www.cidoc-crm.org/cidoc-crm/E55_Type"/>
    <owl:inverseOf rdf:resource="http://iflastandards.info/ns/lrm/lrmoo/R69i_is_physical_form_of"/>
    <rdfs:subPropertyOf rdf:resource="http://www.cidoc-crm.org/cidoc-crm/P2_has_type"/>
    <rdfs:comment xml:lang="en">Quantification: many to many, necessary (1,n:0,n)

Scope note:
This property associates an instance of F3 Manifestation with an instance of E55 Type describing the kind of physical form that characterizes instances of F5 Item carrying this F3 Manifestation.
In the case of instances of manifestations intended to be rendered by mediation (such as with electronic devices), the form also indicates the kind of equipment and software tools necessary.

Examples:
- The publication entitled ‘A clockwork orange’ by Anthony Burgess, published by Penguin Books Ltd in 2008, identified by ISBN ‘0141037229’ (F3) has physical form Printed book (E55).
- The sound recording entitled ‘The Glory (????) of the human voice’, identified by label and label number ‘RCA Victor Gold Seal GD61175’, containing recordings of musical works performed by Florence Foster Jenkins (F3) has physical form Compact Disc (E55).
- The photograph of Billie Holiday by Carl Van Vechten dated 23 March 1949, owned by the Library of Congress and identified by call number LOT 12735, no. 524 [P&amp;P] (F3) has physical form Gelatin silver print (E55).
- The Long Play record entitled ‘Help!’ by The Beatles, released by Parlophone, 6 August 1965, with catalogue number PMC1255 (F3) has physical form Vinyl Long Play record (E55).
- The ebook ‘Christianity: the first three thousand years’ by Diarmaid MacCulloch published by Viking in 2010 and identified by ISBN ‘978-1-101-18999-3’ (F3) has physical form Digital file in EPUB format for Kobo ebook reader (E55).
</rdfs:comment>
  </owl:ObjectProperty>
  <owl:ObjectProperty rdf:about="R69i_is_physical_form_of">
    <rdfs:label xml:lang="en">R69i is physical form of</rdfs:label>
    <skos:notation>R69i</skos:notation>
    <skos:prefLabel xml:lang="en">is physical form of</skos:prefLabel>
    <rdfs:domain rdf:resource="http://www.cidoc-crm.org/cidoc-crm/E55_Type"/>
    <rdfs:range rdf:resource="http://iflastandards.info/ns/lrm/lrmoo/F3_Manifestation"/>
    <owl:inverseOf rdf:resource="http://iflastandards.info/ns/lrm/lrmoo/R69_has_physical_form"/>
    <rdfs:subPropertyOf rdf:resource="http://www.cidoc-crm.org/cidoc-crm/P2i_is_type_of"/>
    <rdfs:comment xml:lang="en">Quantification of the inverse property: many to many, necessary (1,n:0,n)

Scope note of the inverse property:
This property associates an instance of F3 Manifestation with an instance of E55 Type describing the kind of physical form that characterizes instances of F5 Item carrying this F3 Manifestation.
In the case of instances of manifestations intended to be rendered by mediation (such as with electronic devices), the form also indicates the kind of equipment and software tools necessary.

Examples of the inverse property:
- The publication entitled ‘A clockwork orange’ by Anthony Burgess, published by Penguin Books Ltd in 2008, identified by ISBN ‘0141037229’ (F3) has physical form Printed book (E55).
- The sound recording entitled ‘The Glory (????) of the human voice’, identified by label and label number ‘RCA Victor Gold Seal GD61175’, containing recordings of musical works performed by Florence Foster Jenkins (F3) has physical form Compact Disc (E55).
- The photograph of Billie Holiday by Carl Van Vechten dated 23 March 1949, owned by the Library of Congress and identified by call number LOT 12735, no. 524 [P&amp;P] (F3) has physical form Gelatin silver print (E55).
- The Long Play record entitled ‘Help!’ by The Beatles, released by Parlophone, 6 August 1965, with catalogue number PMC1255 (F3) has physical form Vinyl Long Play record (E55).
- The ebook ‘Christianity: the first three thousand years’ by Diarmaid MacCulloch published by Viking in 2010 and identified by ISBN ‘978-1-101-18999-3’ (F3) has physical form Digital file in EPUB format for Kobo ebook reader (E55).
</rdfs:comment>
  </owl:ObjectProperty>
  <owl:ObjectProperty rdf:about="R70_has_dimension">
    <rdfs:label xml:lang="en">R70 has dimension</rdfs:label>
    <skos:notation>R70</skos:notation>
    <skos:prefLabel xml:lang="en">has dimension</skos:prefLabel>
    <rdfs:domain rdf:resource="http://iflastandards.info/ns/lrm/lrmoo/F3_Manifestation"/>
    <rdfs:range rdf:resource="http://www.cidoc-crm.org/cidoc-crm/E54_Dimension"/>
    <owl:inverseOf rdf:resource="http://iflastandards.info/ns/lrm/lrmoo/R70i_is_dimension_of"/>
    <rdfs:subPropertyOf rdf:resource="http://www.cidoc-crm.org/cidoc-crm/P43_has_dimension"/>
    <rdfs:comment xml:lang="en">Quantification: one to many, necessary, dependent (1,n:1,1)

Scope note:
This property associates an instance of F3 Manifestation with an instance of E54 Dimension that describes aspects of its symbolic content, such as word counts, or describes the kind of physical form that characterizes instances of F5 Item carrying this F3 Manifestation, such as number of pages.
This inference is an induction along the path that can be modelled as: F3 Manifestation. R7i is exemplified by: F5 Item. P43 has dimension (is dimension of): E54 Dimension.
It can happen that a given item, or subset of items, originally produced, or intended to be produced, with a certain value for a particular kind of dimension, has a different value for this kind of dimension by accident. This fact should be recorded as a property of F5 Item, and not of F3 Manifestation.

Examples:
- The publication (printed book) entitled ‘Functional Requirements for Bibliographic Records: final report’, published by K. G. Saur in 1998, identified by ISBN ‘3-598-11382-X’ (F3) has dimension height (E54) [which has value (P90) 24 (E60) and has unit (P91) cm (E58)].
- The publication (printed book) entitled ‘A clockwork orange’ by Anthony Burgess, published by Penguin Books Ltd in 2008, identified by ISBN ‘0141037229’ (F3) has dimension number of pages (E54) [which has value (P90) 176 (E60)].
- The publication (Blu-ray box set) entitled ‘Marvel Agents of S.H.I.E.L.D. the Complete Fourth Season’ produced by abc Studios, released in 2018 and identified by EAN ‘8717418521622’ (F3) has dimension number of discs (E54) [which has value (P90) 6 (E60)].
- The jigsaw puzzle entitled ‘Map of the New York city subway system’, designed by Stephen J. Voorhies and released around 1954 by the Union Dimes Savings Bank (F3) has dimension length and height (E54) [which has note (P3) ‘46 x 29 cm’ (E62)].
- The jigsaw puzzle entitled ‘Map of the New York city subway system’, designed by Stephen J. Voorhies and released around 1954 by the Union Dimes Savings Bank (F3) has dimension number of pieces (E54) [which has value (P90) 76 (E60)].
</rdfs:comment>
  </owl:ObjectProperty>
  <owl:ObjectProperty rdf:about="R70i_is_dimension_of">
    <rdfs:label xml:lang="en">R70i is dimension of</rdfs:label>
    <skos:notation>R70i</skos:notation>
    <skos:prefLabel xml:lang="en">is dimension of</skos:prefLabel>
    <rdfs:domain rdf:resource="http://www.cidoc-crm.org/cidoc-crm/E54_Dimension"/>
    <rdfs:range rdf:resource="http://iflastandards.info/ns/lrm/lrmoo/F3_Manifestation"/>
    <owl:inverseOf rdf:resource="http://iflastandards.info/ns/lrm/lrmoo/R70_has_dimension"/>
    <rdfs:subPropertyOf rdf:resource="http://www.cidoc-crm.org/cidoc-crm/P43i_is_dimension_of"/>
    <rdfs:comment xml:lang="en">Quantification of the inverse property: one to many, necessary, dependent (1,n:1,1)

Scope note of the inverse property:
This property associates an instance of F3 Manifestation with an instance of E54 Dimension that describes aspects of its symbolic content, such as word counts, or describes the kind of physical form that characterizes instances of F5 Item carrying this F3 Manifestation, such as number of pages.
This inference is an induction along the path that can be modelled as: F3 Manifestation. R7i is exemplified by: F5 Item. P43 has dimension (is dimension of): E54 Dimension.
It can happen that a given item, or subset of items, originally produced, or intended to be produced, with a certain value for a particular kind of dimension, has a different value for this kind of dimension by accident. This fact should be recorded as a property of F5 Item, and not of F3 Manifestation.

Examples of the inverse property:
- The publication (printed book) entitled ‘Functional Requirements for Bibliographic Records: final report’, published by K. G. Saur in 1998, identified by ISBN ‘3-598-11382-X’ (F3) has dimension height (E54) [which has value (P90) 24 (E60) and has unit (P91) cm (E58)].
- The publication (printed book) entitled ‘A clockwork orange’ by Anthony Burgess, published by Penguin Books Ltd in 2008, identified by ISBN ‘0141037229’ (F3) has dimension number of pages (E54) [which has value (P90) 176 (E60)].
- The publication (Blu-ray box set) entitled ‘Marvel Agents of S.H.I.E.L.D. the Complete Fourth Season’ produced by abc Studios, released in 2018 and identified by EAN ‘8717418521622’ (F3) has dimension number of discs (E54) [which has value (P90) 6 (E60)].
- The jigsaw puzzle entitled ‘Map of the New York city subway system’, designed by Stephen J. Voorhies and released around 1954 by the Union Dimes Savings Bank (F3) has dimension length and height (E54) [which has note (P3) ‘46 x 29 cm’ (E62)].
- The jigsaw puzzle entitled ‘Map of the New York city subway system’, designed by Stephen J. Voorhies and released around 1954 by the Union Dimes Savings Bank (F3) has dimension number of pieces (E54) [which has value (P90) 76 (E60)].
</rdfs:comment>
  </owl:ObjectProperty>
  <owl:ObjectProperty rdf:about="R71_has_part">
    <rdfs:label xml:lang="en">R71 has part</rdfs:label>
    <skos:notation>R71</skos:notation>
    <skos:prefLabel xml:lang="en">has part</skos:prefLabel>
    <rdfs:domain rdf:resource="http://iflastandards.info/ns/lrm/lrmoo/F3_Manifestation"/>
    <rdfs:range rdf:resource="http://iflastandards.info/ns/lrm/lrmoo/F3_Manifestation"/>
    <owl:inverseOf rdf:resource="http://iflastandards.info/ns/lrm/lrmoo/R71i_is_part_of"/>
    <rdfs:subPropertyOf rdf:resource="http://www.cidoc-crm.org/cidoc-crm/P148_has_component"/>
    <rdfs:comment xml:lang="en">Quantification: many to many (0,n:0,n)

Scope note:
This property associates an instance of F3 Manifestation with a structural part of it that is itself an instance of F3 Manifestation. This property is transitive, asymmetric and irreflexive.

Examples:
- The publication (set of 3 books) containing J. R. R. Tolkien’s ‘The Lord of the rings’ identified by ISBN ‘0618260587’ (F3) has part the publication containing J. R. R. Tolkien’s ‘The two towers’ identified by ISBN ‘0618260595’ (F3).
- The compact disc publication issued by Deutsche Grammophon in 1998 and consisting of a recording of Richard Wagner’s ‘Der fliegende Holländer’ as performed in 1991 by Plácido Domingo, Cheryl Studer et al., and conducted by Giuseppe Sinopoli (F3) has part a publication consisting of the printed program notes and libretto (F3).
- The compact disc publication issued as a 2-CD set identified as ‘M2K 42270’ by CBS Records in 1987 and consisting of recordings of J. S. Bach’s concertos for keyboard/clavier and strings performed by Glenn Gould (F3) has part the compact disc publication identified as ‘DIDC 10370’ consisting of the Glenn Gould recordings of Bach’s ‘Concertos nos. 1-4’ (F3).
</rdfs:comment>
  </owl:ObjectProperty>
  <owl:ObjectProperty rdf:about="R71i_is_part_of">
    <rdfs:label xml:lang="en">R71i is part of</rdfs:label>
    <skos:notation>R71i</skos:notation>
    <skos:prefLabel xml:lang="en">is part of</skos:prefLabel>
    <rdfs:domain rdf:resource="http://iflastandards.info/ns/lrm/lrmoo/F3_Manifestation"/>
    <rdfs:range rdf:resource="http://iflastandards.info/ns/lrm/lrmoo/F3_Manifestation"/>
    <owl:inverseOf rdf:resource="http://iflastandards.info/ns/lrm/lrmoo/R71_has_part"/>
    <rdfs:subPropertyOf rdf:resource="http://www.cidoc-crm.org/cidoc-crm/P148i_is_component_of"/>
    <rdfs:comment xml:lang="en">Quantification of the inverse property: many to many (0,n:0,n)

Scope note of the inverse property:
This property associates an instance of F3 Manifestation with a structural part of it that is itself an instance of F3 Manifestation. This property is transitive, asymmetric and irreflexive.

Examples of the inverse property:
- The publication (set of 3 books) containing J. R. R. Tolkien’s ‘The Lord of the rings’ identified by ISBN ‘0618260587’ (F3) has part the publication containing J. R. R. Tolkien’s ‘The two towers’ identified by ISBN ‘0618260595’ (F3).
- The compact disc publication issued by Deutsche Grammophon in 1998 and consisting of a recording of Richard Wagner’s ‘Der fliegende Holländer’ as performed in 1991 by Plácido Domingo, Cheryl Studer et al., and conducted by Giuseppe Sinopoli (F3) has part a publication consisting of the printed program notes and libretto (F3).
- The compact disc publication issued as a 2-CD set identified as ‘M2K 42270’ by CBS Records in 1987 and consisting of recordings of J. S. Bach’s concertos for keyboard/clavier and strings performed by Glenn Gould (F3) has part the compact disc publication identified as ‘DIDC 10370’ consisting of the Glenn Gould recordings of Bach’s ‘Concertos nos. 1-4’ (F3).
</rdfs:comment>
  </owl:ObjectProperty>
  <owl:ObjectProperty rdf:about="R73_takes_representative_attribute_from">
    <rdfs:label xml:lang="en">R73 takes representative attribute from</rdfs:label>
    <skos:notation>R73</skos:notation>
    <skos:prefLabel xml:lang="en">takes representative attribute from</skos:prefLabel>
    <rdfs:domain rdf:resource="http://iflastandards.info/ns/lrm/lrmoo/F1_Work"/>
    <rdfs:range rdf:resource="http://iflastandards.info/ns/lrm/lrmoo/F2_Expression"/>
    <owl:inverseOf rdf:resource="http://iflastandards.info/ns/lrm/lrmoo/R73i_bears_representative_attribute_for"/>
    <rdfs:comment xml:lang="en">Quantification: one to many, necessary (1,n:0,1)

Shortcut Of: F1 Work. P140i was attributed by: E13 Attribute Assignment. P16 uses specific object: F2 Expression

Scope note:
This property associates an instance of F1 Work with instances of F2 Expression that bear attributes which are used to characterize the work. The instance of F2 Expression in question must be one that realizes that instance of F1 Work. An instance of F2 Expression may or may not serve as source of representative expression attributes for its associated instance of F1 Work. If it does, it may provide one attribute or many. Only one or more than one of the instances of F2 Expression associated with an instance of F1 Work may provide attributes that characterize that instance of F1 Work. The representative expression attributes can all come from the same expression or from more than one expressions.

Examples:
- The work ‘Reading for life, a first book for adults and their tutors’ by Virginia French Allen (F1) takes representative attribute from the expression first published in 1987 by Spring Institute for International Studies with ISBN ‘094072300X’ (F2). [One attribute is the value for intended audience, which is adult literacy learners in the English language, another attribute is the language English.]
- The expression of the work ‘Piglet has a bath’ by A. A. Milne, with illustrations by Ernest H. Shepard, realised in the edition published on sealed plastic pages by Dutton Children’s Books in 1998 with ISBN ‘0525460926’ (F2) bears representative attribute for the work ‘Piglet has a bath’ by A. A. Milne (F1). [One attribute is the language English; another is the value for intended audience, which is children.]
- The work ‘Fugue in G Minor, BWV 1000’ by Johann Sebastian Bach (F1) takes representative attribute from the original expression (F2) (as composed around 1723). [The attribute is lute as the mode of performance; it is now mostly performed on the guitar.]
</rdfs:comment>
  </owl:ObjectProperty>
  <owl:ObjectProperty rdf:about="R73i_bears_representative_attribute_for">
    <rdfs:label xml:lang="en">R73i bears representative attribute for</rdfs:label>
    <skos:notation>R73i</skos:notation>
    <skos:prefLabel xml:lang="en">bears representative attribute for</skos:prefLabel>
    <rdfs:domain rdf:resource="http://iflastandards.info/ns/lrm/lrmoo/F2_Expression"/>
    <rdfs:range rdf:resource="http://iflastandards.info/ns/lrm/lrmoo/F1_Work"/>
    <owl:inverseOf rdf:resource="http://iflastandards.info/ns/lrm/lrmoo/R73_takes_representative_attribute_from"/>
    <rdfs:comment xml:lang="en">Quantification of the inverse property: one to many, necessary (1,n:0,1)

Shortcut Of of the inverse property: F1 Work. P140i was attributed by: E13 Attribute Assignment. P16 uses specific object: F2 Expression

Scope note of the inverse property:
This property associates an instance of F1 Work with instances of F2 Expression that bear attributes which are used to characterize the work. The instance of F2 Expression in question must be one that realizes that instance of F1 Work. An instance of F2 Expression may or may not serve as source of representative expression attributes for its associated instance of F1 Work. If it does, it may provide one attribute or many. Only one or more than one of the instances of F2 Expression associated with an instance of F1 Work may provide attributes that characterize that instance of F1 Work. The representative expression attributes can all come from the same expression or from more than one expressions.

Examples of the inverse property:
- The work ‘Reading for life, a first book for adults and their tutors’ by Virginia French Allen (F1) takes representative attribute from the expression first published in 1987 by Spring Institute for International Studies with ISBN ‘094072300X’ (F2). [One attribute is the value for intended audience, which is adult literacy learners in the English language, another attribute is the language English.]
- The expression of the work ‘Piglet has a bath’ by A. A. Milne, with illustrations by Ernest H. Shepard, realised in the edition published on sealed plastic pages by Dutton Children’s Books in 1998 with ISBN ‘0525460926’ (F2) bears representative attribute for the work ‘Piglet has a bath’ by A. A. Milne (F1). [One attribute is the language English; another is the value for intended audience, which is children.]
- The work ‘Fugue in G Minor, BWV 1000’ by Johann Sebastian Bach (F1) takes representative attribute from the original expression (F2) (as composed around 1723). [The attribute is lute as the mode of performance; it is now mostly performed on the guitar.]
</rdfs:comment>
  </owl:ObjectProperty>
  <owl:ObjectProperty rdf:about="R74_uses_expression_of">
    <rdfs:label xml:lang="en">R74 uses expression of</rdfs:label>
    <skos:notation>R74</skos:notation>
    <skos:prefLabel xml:lang="en">uses expression of</skos:prefLabel>
    <rdfs:domain rdf:resource="http://iflastandards.info/ns/lrm/lrmoo/F1_Work"/>
    <rdfs:range rdf:resource="http://iflastandards.info/ns/lrm/lrmoo/F1_Work"/>
    <owl:inverseOf rdf:resource="http://iflastandards.info/ns/lrm/lrmoo/R74i_has_expression_used_in"/>
    <rdfs:subPropertyOf rdf:resource="http://www.cidoc-crm.org/cidoc-crm/P130_shows_features_of"/>
    <rdfs:comment xml:lang="en">Quantification: many to many (0,n:0,n)

Scope note:
This property associates an instance of F1 Work with another instance of F1 Work where all expressions of the former will include some expression of the latter. This property is not transitive. It is irreflexive. This property represents the generalized relationship between works that is described at the expression level using R75 incorporates (is incorporated in).

Examples:
- Ludwig van Beethoven’s ‘Symphony No. 9’ (F1) uses expression of the poem ‘An die Freude’ by Friedrich Schiller (F1).
- Franz Schubert’s kunstlied ‘Erlkönig’ (F1) uses expression of the poem ‘Erlkönig’ by Johann Wolfgang von Goethe (F1).
- The symphonic poem ‘Vltava’ by Bedřich Smetana (F1) uses expression of the melody ‘La Mantovana’ attributed to Giuseppe Cenci (F1).
</rdfs:comment>
  </owl:ObjectProperty>
  <owl:ObjectProperty rdf:about="R74i_has_expression_used_in">
    <rdfs:label xml:lang="en">R74i has expression used in</rdfs:label>
    <skos:notation>R74i</skos:notation>
    <skos:prefLabel xml:lang="en">has expression used in</skos:prefLabel>
    <rdfs:domain rdf:resource="http://iflastandards.info/ns/lrm/lrmoo/F1_Work"/>
    <rdfs:range rdf:resource="http://iflastandards.info/ns/lrm/lrmoo/F1_Work"/>
    <owl:inverseOf rdf:resource="http://iflastandards.info/ns/lrm/lrmoo/R74_uses_expression_of"/>
    <rdfs:subPropertyOf rdf:resource="http://www.cidoc-crm.org/cidoc-crm/P130i_features_are_also_found_on"/>
    <rdfs:comment xml:lang="en">Quantification of the inverse property: many to many (0,n:0,n)

Scope note of the inverse property:
This property associates an instance of F1 Work with another instance of F1 Work where all expressions of the former will include some expression of the latter. This property is not transitive. It is irreflexive. This property represents the generalized relationship between works that is described at the expression level using R75 incorporates (is incorporated in).

Examples of the inverse property:
- Ludwig van Beethoven’s ‘Symphony No. 9’ (F1) uses expression of the poem ‘An die Freude’ by Friedrich Schiller (F1).
- Franz Schubert’s kunstlied ‘Erlkönig’ (F1) uses expression of the poem ‘Erlkönig’ by Johann Wolfgang von Goethe (F1).
- The symphonic poem ‘Vltava’ by Bedřich Smetana (F1) uses expression of the melody ‘La Mantovana’ attributed to Giuseppe Cenci (F1).
</rdfs:comment>
  </owl:ObjectProperty>
  <owl:ObjectProperty rdf:about="R75_incorporates">
    <rdfs:label xml:lang="en">R75 incorporates</rdfs:label>
    <skos:notation>R75</skos:notation>
    <skos:prefLabel xml:lang="en">incorporates</skos:prefLabel>
    <rdfs:domain rdf:resource="http://iflastandards.info/ns/lrm/lrmoo/F2_Expression"/>
    <rdfs:range rdf:resource="http://iflastandards.info/ns/lrm/lrmoo/F2_Expression"/>
    <owl:inverseOf rdf:resource="http://iflastandards.info/ns/lrm/lrmoo/R75i_is_incorporated_in"/>
    <rdfs:subPropertyOf rdf:resource="http://www.cidoc-crm.org/cidoc-crm/P165_incorporates"/>
    <rdfs:comment xml:lang="en">Quantification: many to many (0,n:0,n)

Scope note:
This property associates an instance of F2 Expression with an instance of F2 Expression that is an integral part of the first, but where the latter realises a different instance of F1 Work from the first. This property is transitive, asymmetric and irreflexive.

Examples:
- The 1964 recording of Beethoven’s ‘Symphony No. 9’ by Leonard Bernstein and the New York Philharmonic (F2) incorporates the German text of the poem ‘An die Freude’ by Friedrich Schiller (F2).
- Franz Schubert’s score for the kunstlied ‘Erlkönig’ that was created in 1815 (F2) incorporates the German text of the poem ‘Erlkönig’ by Johann Wolfgang von Goethe (F2).
- Pyotr Ilyich Tchaikovsky’s graduation cantata performed by Leslie Head and the Kensington Symphony Orchestra in 1978 (F2) incorporates a Russian translation of the poem ‘An die Freude’ by Friedrich Schiller (F2).
</rdfs:comment>
  </owl:ObjectProperty>
  <owl:ObjectProperty rdf:about="R75i_is_incorporated_in">
    <rdfs:label xml:lang="en">R75i is incorporated in</rdfs:label>
    <skos:notation>R75i</skos:notation>
    <skos:prefLabel xml:lang="en">is incorporated in</skos:prefLabel>
    <rdfs:domain rdf:resource="http://iflastandards.info/ns/lrm/lrmoo/F2_Expression"/>
    <rdfs:range rdf:resource="http://iflastandards.info/ns/lrm/lrmoo/F2_Expression"/>
    <owl:inverseOf rdf:resource="http://iflastandards.info/ns/lrm/lrmoo/R75_incorporates"/>
    <rdfs:subPropertyOf rdf:resource="http://www.cidoc-crm.org/cidoc-crm/P165i_is_incorporated_in"/>
    <rdfs:comment xml:lang="en">Quantification of the inverse property: many to many (0,n:0,n)

Scope note of the inverse property:
This property associates an instance of F2 Expression with an instance of F2 Expression that is an integral part of the first, but where the latter realises a different instance of F1 Work from the first. This property is transitive, asymmetric and irreflexive.

Examples of the inverse property:
- The 1964 recording of Beethoven’s ‘Symphony No. 9’ by Leonard Bernstein and the New York Philharmonic (F2) incorporates the German text of the poem ‘An die Freude’ by Friedrich Schiller (F2).
- Franz Schubert’s score for the kunstlied ‘Erlkönig’ that was created in 1815 (F2) incorporates the German text of the poem ‘Erlkönig’ by Johann Wolfgang von Goethe (F2).
- Pyotr Ilyich Tchaikovsky’s graduation cantata performed by Leslie Head and the Kensington Symphony Orchestra in 1978 (F2) incorporates a Russian translation of the poem ‘An die Freude’ by Friedrich Schiller (F2).
</rdfs:comment>
  </owl:ObjectProperty>
  <owl:ObjectProperty rdf:about="R76_is_derivative_of">
    <rdfs:label xml:lang="en">R76 is derivative of</rdfs:label>
    <skos:notation>R76</skos:notation>
    <skos:prefLabel xml:lang="en">is derivative of</skos:prefLabel>
    <rdfs:domain rdf:resource="http://iflastandards.info/ns/lrm/lrmoo/F2_Expression"/>
    <rdfs:range rdf:resource="http://iflastandards.info/ns/lrm/lrmoo/F2_Expression"/>
    <owl:inverseOf rdf:resource="http://iflastandards.info/ns/lrm/lrmoo/R76i_has_derivative"/>
    <rdfs:subPropertyOf rdf:resource="http://www.cidoc-crm.org/cidoc-crm/P130_shows_features_of"/>
    <rdfs:comment xml:lang="en">Quantification: many to many (0,n:0,n)

Scope note:
This property associates an instance of F2 Expression with another instance of F2 Expression which was its source or one of its sources. This property is not transitive. It is asymmetric and irreflexive.
This property is also a shortcut of the fully developed path: F2 Expression (1). P16i was used for: F28 Expression Creation. R17 created: F2 Expression (2).

Examples:
- Elisabeth van Bebber’s German text of Agatha Christie’s ‘Murder on the Orient Express’ (F2) is derivative of the original text written by Agatha Christie for the novel (F2) with has type Translation (E55).
- The text of Agatha Christie’s ‘Murder on the Orient Express Abridged’ (as published by HarperCollins) (F2) is derivative of the original text written by Agatha Christie for the novel (F2) with has type Abridgement (E55).
- The musical score for Dmitry Sitkovetsky’s ‘Goldberg Variations’ arranged for string (F2) is derivative of the musical score for Johann Sebastian Bach’s ‘Goldberg Variations’ (F2) with has type Arrangement (E55).
- The score for Beethoven’s 9th Symphony edited by Jonathan Del Mar (F2) is derivation of Beethoven’s original score for the 9th Symphony (F2) with has type Revision (E55).

Properties:
- R76.1 has type: 
  Scope note:
    This property allows for specifying the kind of derivation, such as translation, revision, etc.
</rdfs:comment>
  </owl:ObjectProperty>
  <owl:ObjectProperty rdf:about="R76i_has_derivative">
    <rdfs:label xml:lang="en">R76i has derivative</rdfs:label>
    <skos:notation>R76i</skos:notation>
    <skos:prefLabel xml:lang="en">has derivative</skos:prefLabel>
    <rdfs:domain rdf:resource="http://iflastandards.info/ns/lrm/lrmoo/F2_Expression"/>
    <rdfs:range rdf:resource="http://iflastandards.info/ns/lrm/lrmoo/F2_Expression"/>
    <owl:inverseOf rdf:resource="http://iflastandards.info/ns/lrm/lrmoo/R76_is_derivative_of"/>
    <rdfs:subPropertyOf rdf:resource="http://www.cidoc-crm.org/cidoc-crm/P130i_features_are_also_found_on"/>
    <rdfs:comment xml:lang="en">Quantification of the inverse property: many to many (0,n:0,n)

Scope note of the inverse property:
This property associates an instance of F2 Expression with another instance of F2 Expression which was its source or one of its sources. This property is not transitive. It is asymmetric and irreflexive.
This property is also a shortcut of the fully developed path: F2 Expression (1). P16i was used for: F28 Expression Creation. R17 created: F2 Expression (2).

Examples of the inverse property:
- Elisabeth van Bebber’s German text of Agatha Christie’s ‘Murder on the Orient Express’ (F2) is derivative of the original text written by Agatha Christie for the novel (F2) with has type Translation (E55).
- The text of Agatha Christie’s ‘Murder on the Orient Express Abridged’ (as published by HarperCollins) (F2) is derivative of the original text written by Agatha Christie for the novel (F2) with has type Abridgement (E55).
- The musical score for Dmitry Sitkovetsky’s ‘Goldberg Variations’ arranged for string (F2) is derivative of the musical score for Johann Sebastian Bach’s ‘Goldberg Variations’ (F2) with has type Arrangement (E55).
- The score for Beethoven’s 9th Symphony edited by Jonathan Del Mar (F2) is derivation of Beethoven’s original score for the 9th Symphony (F2) with has type Revision (E55).
</rdfs:comment>
  </owl:ObjectProperty>
  <owl:ObjectProperty rdf:about="R77_accompanies_or_complements">
    <rdfs:label xml:lang="en">R77 accompanies or complements</rdfs:label>
    <skos:notation>R77</skos:notation>
    <skos:prefLabel xml:lang="en">accompanies or complements</skos:prefLabel>
    <rdfs:domain rdf:resource="http://iflastandards.info/ns/lrm/lrmoo/F1_Work"/>
    <rdfs:range rdf:resource="http://iflastandards.info/ns/lrm/lrmoo/F1_Work"/>
    <owl:inverseOf rdf:resource="http://iflastandards.info/ns/lrm/lrmoo/R77i_is_accompanied_or_complemented_by"/>
    <rdfs:comment xml:lang="en">Quantification: many to many (0,n:0,n)

Shortcut Of: F1 Work. P19i was made for: E7 Activity. P19 was intended use of: F1 Work

Scope note:
This property associates one instance of F1 Work with another instance of F1 Work which is intended to accompany it or to function as a complement for it. This property is neither transitive nor intransitive. It is generally not symmetric and it is irreflexive.
In many but not all cases, one of the instances of F1 Work is primary and can be used without the other work, while the other is secondary and depends on the first work (such as a work that is a concordance for another work).
In some cases a work may have been created to accompany or complement a specific expression of another work. The link to the source expression can be indicated using the property P16 used specific object (was used for) using the path: F1 Work(1). R3 is realised in: F2 Expression(1). P16i was used for: F27 Work Creation. R16 created: F1 Work(2).

Examples:
- Leigh Lowe’s ‘Prima Latina: an introduction to Christian Latin. Teacher manual’ (F1) accompanies or complements Leigh Lowe’s ‘Prima Latina: an introduction to Christian Latin. Student book’ (F1).
- Eric Gill’s set of illustrations for the Song of Songs (F1) accompanies or complements the ‘Song of Songs’ in the 1931 publication by the Cranach Press (F1).
- The periodical ‘Applied economics quarterly’ (ISSN 1611-6607) (F1) is accompanied or complemented by the periodical ‘Applied economics quarterly. Supplement’ (ISSN 1612-2127) (F1).
- The novel ‘Le chevalier au lion’ by Chrétien de Troyes (F1) is accompanied or complemented by the concordance created by Pascal Bonnefois and Marie-Louise Ollier ‘Yvain ou Le chevalier au lion : concordance lemmatisée’ (F1). [The concordance is specifically based on the 1960 edition of the novel by Mario Roques.]
</rdfs:comment>
  </owl:ObjectProperty>
  <owl:ObjectProperty rdf:about="R77i_is_accompanied_or_complemented_by">
    <rdfs:label xml:lang="en">R77i is accompanied or complemented by</rdfs:label>
    <skos:notation>R77i</skos:notation>
    <skos:prefLabel xml:lang="en">is accompanied or complemented by</skos:prefLabel>
    <rdfs:domain rdf:resource="http://iflastandards.info/ns/lrm/lrmoo/F1_Work"/>
    <rdfs:range rdf:resource="http://iflastandards.info/ns/lrm/lrmoo/F1_Work"/>
    <owl:inverseOf rdf:resource="http://iflastandards.info/ns/lrm/lrmoo/R77_accompanies_or_complements"/>
    <rdfs:comment xml:lang="en">Quantification of the inverse property: many to many (0,n:0,n)

Shortcut Of of the inverse property: F1 Work. P19i was made for: E7 Activity. P19 was intended use of: F1 Work

Scope note of the inverse property:
This property associates one instance of F1 Work with another instance of F1 Work which is intended to accompany it or to function as a complement for it. This property is neither transitive nor intransitive. It is generally not symmetric and it is irreflexive.
In many but not all cases, one of the instances of F1 Work is primary and can be used without the other work, while the other is secondary and depends on the first work (such as a work that is a concordance for another work).
In some cases a work may have been created to accompany or complement a specific expression of another work. The link to the source expression can be indicated using the property P16 used specific object (was used for) using the path: F1 Work(1). R3 is realised in: F2 Expression(1). P16i was used for: F27 Work Creation. R16 created: F1 Work(2).

Examples of the inverse property:
- Leigh Lowe’s ‘Prima Latina: an introduction to Christian Latin. Teacher manual’ (F1) accompanies or complements Leigh Lowe’s ‘Prima Latina: an introduction to Christian Latin. Student book’ (F1).
- Eric Gill’s set of illustrations for the Song of Songs (F1) accompanies or complements the ‘Song of Songs’ in the 1931 publication by the Cranach Press (F1).
- The periodical ‘Applied economics quarterly’ (ISSN 1611-6607) (F1) is accompanied or complemented by the periodical ‘Applied economics quarterly. Supplement’ (ISSN 1612-2127) (F1).
- The novel ‘Le chevalier au lion’ by Chrétien de Troyes (F1) is accompanied or complemented by the concordance created by Pascal Bonnefois and Marie-Louise Ollier ‘Yvain ou Le chevalier au lion : concordance lemmatisée’ (F1). [The concordance is specifically based on the 1960 edition of the novel by Mario Roques.]
</rdfs:comment>
  </owl:ObjectProperty>
  <owl:ObjectProperty rdf:about="R78_has_alternate">
    <rdfs:label xml:lang="en">R78 has alternate</rdfs:label>
    <skos:notation>R78</skos:notation>
    <skos:prefLabel xml:lang="en">has alternate</skos:prefLabel>
    <rdfs:domain rdf:resource="http://iflastandards.info/ns/lrm/lrmoo/F3_Manifestation"/>
    <rdfs:range rdf:resource="http://iflastandards.info/ns/lrm/lrmoo/F3_Manifestation"/>
    <rdfs:comment xml:lang="en">Quantification: many to many (0,n:0,n)

Inverse Shortcut Of: F3 Manifestation. R4 embodies: F2 Expression. R4i is embodied by: F3 Manifestation

Scope note:
This property associates one instance of F3 Manifestation with another instance of F3 Manifestation that exemplifies the same instance of F2 Expression, when the two instances of F3 Manifestation can be used as alternatives for each other in particular use cases. This property is transitive and symmetric. It is irreflexive.
The alternative manifestations may be in the same physical form, for example, simultaneous publications in different markets. More frequently, the alternative relationship is established when the alternative manifestations are in different physical forms, designed to enable use of the same content with different playback equipment (such as a DVD and Blu-ray disc version of the same videorecording).

Examples:
- Agatha Christie’s ‘The Sittaford Mystery’ published in 1931 in the UK by William Collins &amp; Sons (F3) has alternate the simultaneous US edition published as ‘The Murder at Hazelmoor’ by Dodd, Mead &amp; Co. (F3).
- The LP release of the punk rock band the Soviettes’ album titled ‘LP III’ (F3) has alternate the CD release of the punk rock band the Soviettes’ album titled ‘LP III’ (F3).
</rdfs:comment>
  </owl:ObjectProperty>
  <owl:ObjectProperty rdf:about="R79_has_representative_expression_attribute">
    <rdfs:label xml:lang="en">R79 has representative expression attribute</rdfs:label>
    <skos:notation>R79</skos:notation>
    <skos:prefLabel xml:lang="en">has representative expression attribute</skos:prefLabel>
    <rdfs:domain rdf:resource="http://iflastandards.info/ns/lrm/lrmoo/F1_Work"/>
    <rdfs:range rdf:resource="http://www.cidoc-crm.org/cidoc-crm/E55_Type"/>
    <owl:inverseOf rdf:resource="http://iflastandards.info/ns/lrm/lrmoo/R79i_is_representative_expression_attribute_of"/>
    <rdfs:subPropertyOf rdf:resource="http://www.cidoc-crm.org/cidoc-crm/P2_has_type"/>
    <rdfs:comment xml:lang="en">Quantification: many to many (0,n:0,n)

Scope note:
This property associates an instance of F1 Work with an instance of E55 Type that describes a category of attribute that is considered essential in characterizing instances of F1 Work. The types of interest will vary depending on the kind of work.
The value of the attribute is considered representative of the instance of F1 Work. It is normally inferred from the values attributed to instances of F2 Expression that realize the work and that are considered canonical or best representative of the work. The values may also be assigned from characteristics abstracted from a more or less nebulous network of similar expressions. There is no requirement to precisely identify one or more expressions which serve as sources for the values of the types serving as representative expression attributes; however, if this is known, an instance of F2 Expression considered representative of an F1 Work may be related to the instance of F1 Work using the R73 takes representative attribute from (bears representative attribute for) property.

Examples:
- The work ‘Reading for life, a first book for adults and their tutors’ by Virginia French Allen (F1) has representative expression attribute language ‘English’ (E56).
- The work ‘Piglet has a bath’ by A. A. Milne (F1) has representative expression attribute intended audience ‘children’ (E55).
- The work ‘Fugue in G Minor, BWV 1000’ by Johann Sebastian Bach (F1) has representative expression attribute medium of performance ‘lute’ (E55). [The original 1723 composition was for lute; it is now mostly performed on the guitar.]
</rdfs:comment>
  </owl:ObjectProperty>
  <owl:ObjectProperty rdf:about="R79i_is_representative_expression_attribute_of">
    <rdfs:label xml:lang="en">R79i is representative expression attribute of</rdfs:label>
    <skos:notation>R79i</skos:notation>
    <skos:prefLabel xml:lang="en">is representative expression attribute of</skos:prefLabel>
    <rdfs:domain rdf:resource="http://www.cidoc-crm.org/cidoc-crm/E55_Type"/>
    <rdfs:range rdf:resource="http://iflastandards.info/ns/lrm/lrmoo/F1_Work"/>
    <owl:inverseOf rdf:resource="http://iflastandards.info/ns/lrm/lrmoo/R79_has_representative_expression_attribute"/>
    <rdfs:subPropertyOf rdf:resource="http://www.cidoc-crm.org/cidoc-crm/P2i_is_type_of"/>
    <rdfs:comment xml:lang="en">Quantification of the inverse property: many to many (0,n:0,n)

Scope note of the inverse property:
This property associates an instance of F1 Work with an instance of E55 Type that describes a category of attribute that is considered essential in characterizing instances of F1 Work. The types of interest will vary depending on the kind of work.
The value of the attribute is considered representative of the instance of F1 Work. It is normally inferred from the values attributed to instances of F2 Expression that realize the work and that are considered canonical or best representative of the work. The values may also be assigned from characteristics abstracted from a more or less nebulous network of similar expressions. There is no requirement to precisely identify one or more expressions which serve as sources for the values of the types serving as representative expression attributes; however, if this is known, an instance of F2 Expression considered representative of an F1 Work may be related to the instance of F1 Work using the R73 takes representative attribute from (bears representative attribute for) property.

Examples of the inverse property:
- The work ‘Reading for life, a first book for adults and their tutors’ by Virginia French Allen (F1) has representative expression attribute language ‘English’ (E56).
- The work ‘Piglet has a bath’ by A. A. Milne (F1) has representative expression attribute intended audience ‘children’ (E55).
- The work ‘Fugue in G Minor, BWV 1000’ by Johann Sebastian Bach (F1) has representative expression attribute medium of performance ‘lute’ (E55). [The original 1723 composition was for lute; it is now mostly performed on the guitar.]
</rdfs:comment>
  </owl:ObjectProperty>
  <owl:ObjectProperty rdf:about="R80_performed">
    <rdfs:label xml:lang="en">R80 performed</rdfs:label>
    <skos:notation>R80</skos:notation>
    <skos:prefLabel xml:lang="en">performed</skos:prefLabel>
    <rdfs:domain rdf:resource="http://iflastandards.info/ns/lrm/lrmoo/F31_Performance"/>
    <rdfs:range rdf:resource="http://iflastandards.info/ns/lrm/lrmoo/F1_Work"/>
    <owl:inverseOf rdf:resource="http://iflastandards.info/ns/lrm/lrmoo/R80i_is_performed_in"/>
    <rdfs:subPropertyOf rdf:resource="http://www.cidoc-crm.org/cidoc-crm/P130_shows_features_of"/>
    <rdfs:comment xml:lang="en">Quantification: many to one, necessary (1,1:0,n)

Scope note:
This property associates an instance of F31 Performance with an instance of F1 Work.
The property is used to express the association between an instance of F31 Performance and the instance of F1 Work it conveys.

Examples:
- The performance of ‘Hamlet’ on 17 June 1909 in Berlin, Deutsches Theater, by Alexander Moissi, directed by Max Reinhardt (F31) performed William Shakespeare’s work ‘Hamlet’ (F1).
- The performance (at the Salzburg Festival in 2005) of Verdi’s ‘La Traviata’ that was staged by Willy Decker, directed by Brian Large and featuring Anna Netrebko and Rolando Villazón (F31) performed Giuseppe Verdi’s work ‘La Traviata’ (F1).
- The performance on July 7, 1995 (at the Popes’ Palace in Avignon) of the ballet entitled ‘Rite of spring’ (F31) performed the choreographic work ‘Rite of spring’ by Pina Bausch (F1).
- The Mariinsky Orchestra and Ballet’s performance of Michel Fokine’s choreography and libretto (choreographic work) for Stravinsky’s ‘The Firebird’ at the Mariinsky Theatre in Saint Petersburg, June 2008 (F31) performed Michel Fokine’s choreography and libretto (choreographic work) for Stravinsky’s ‘The Firebird’ (F1).
- The performance of Daniel Humair (drums) and Damien Varaillon (double bass) improvising their ‘Hommage à John Coltrane’ in the Bal Blomet (Paris), on 18 January 2018 (F31) performed Daniel Humair and Damien Varaillon’s work ‘Hommage à John Coltrane’ (F1).
</rdfs:comment>
  </owl:ObjectProperty>
  <owl:ObjectProperty rdf:about="R80i_is_performed_in">
    <rdfs:label xml:lang="en">R80i is performed in</rdfs:label>
    <skos:notation>R80i</skos:notation>
    <skos:prefLabel xml:lang="en">is performed in</skos:prefLabel>
    <rdfs:domain rdf:resource="http://iflastandards.info/ns/lrm/lrmoo/F1_Work"/>
    <rdfs:range rdf:resource="http://iflastandards.info/ns/lrm/lrmoo/F31_Performance"/>
    <owl:inverseOf rdf:resource="http://iflastandards.info/ns/lrm/lrmoo/R80_performed"/>
    <rdfs:subPropertyOf rdf:resource="http://www.cidoc-crm.org/cidoc-crm/P130i_features_are_also_found_on"/>
    <rdfs:comment xml:lang="en">Quantification of the inverse property: many to one, necessary (1,1:0,n)

Scope note of the inverse property:
This property associates an instance of F31 Performance with an instance of F1 Work.
The property is used to express the association between an instance of F31 Performance and the instance of F1 Work it conveys.

Examples of the inverse property:
- The performance of ‘Hamlet’ on 17 June 1909 in Berlin, Deutsches Theater, by Alexander Moissi, directed by Max Reinhardt (F31) performed William Shakespeare’s work ‘Hamlet’ (F1).
- The performance (at the Salzburg Festival in 2005) of Verdi’s ‘La Traviata’ that was staged by Willy Decker, directed by Brian Large and featuring Anna Netrebko and Rolando Villazón (F31) performed Giuseppe Verdi’s work ‘La Traviata’ (F1).
- The performance on July 7, 1995 (at the Popes’ Palace in Avignon) of the ballet entitled ‘Rite of spring’ (F31) performed the choreographic work ‘Rite of spring’ by Pina Bausch (F1).
- The Mariinsky Orchestra and Ballet’s performance of Michel Fokine’s choreography and libretto (choreographic work) for Stravinsky’s ‘The Firebird’ at the Mariinsky Theatre in Saint Petersburg, June 2008 (F31) performed Michel Fokine’s choreography and libretto (choreographic work) for Stravinsky’s ‘The Firebird’ (F1).
- The performance of Daniel Humair (drums) and Damien Varaillon (double bass) improvising their ‘Hommage à John Coltrane’ in the Bal Blomet (Paris), on 18 January 2018 (F31) performed Daniel Humair and Damien Varaillon’s work ‘Hommage à John Coltrane’ (F1).
</rdfs:comment>
  </owl:ObjectProperty>
  <owl:ObjectProperty rdf:about="R81_recorded">
    <rdfs:label xml:lang="en">R81 recorded</rdfs:label>
    <skos:notation>R81</skos:notation>
    <skos:prefLabel xml:lang="en">recorded</skos:prefLabel>
    <rdfs:domain rdf:resource="http://iflastandards.info/ns/lrm/lrmoo/F28_Expression_Creation"/>
    <rdfs:range rdf:resource="http://iflastandards.info/ns/lrm/lrmoo/F31_Performance"/>
    <owl:inverseOf rdf:resource="http://iflastandards.info/ns/lrm/lrmoo/R81i_is_recorded_in"/>
    <rdfs:comment xml:lang="en">Quantification: many to one (0,1:0,n)

Scope note:
This property associates an instance of F28 Expression Creation with an instance of F31 Performance that it records.
This property allows for the documentation of the association that exists between the outcome of an instance of F28 Expression Creation such as a performance recording, and the instance of F31 Performance that it is a recording of. For documenting performances that are more integral and planned parts of an expression creation (such as the recording of a performance solely done for the purpose of audio or video productions), the use of the property P9 consist of (forms part of) is more specific (and appropriate).

Examples:
- The Hyperion production (for CD release) of Angela Hewitt performing the ‘Goldberg Variations’ (F28) recorded Angela Hewitt’s performance of the ‘Goldberg Variations’ in Christuskirche (Berlin) on 14-17 December 2015 (F31).
- The Deutsche Grammophon video production of Verdi’s ‘La Traviata’ from the Salzburg Festival in 2005 (F28) recorded the live performance of ‘La Traviata’ that was staged by Willy Decker, directed by Brian Large and featuring Anna Netrebko and Rolando Villazón (F31).
- The Deutsche Grammophon audio production of Verdi’s ‘La Traviata’ from the Salzburg Festival in 2005 (F28) recorded the live performance of ‘La Traviata’ performed by the Vienna Philharmonic, conducted by Carlo Rizzi featuring Anna Netrebko and Rolando Villazón (F31).
- The Belair production (DVD) produced by François Duplat and directed for video by Denis Calozzi, of Michel Fokine’s choreography and libretto for Stravinsky’s ‘The Firebird’ (F28) recorded the Mariinsky Orchestra and Ballet’s performance of Michel Fokine’s choreography and libretto (choreographic work) for Stravinsky’s ‘The Firebird’, at the Mariinsky Theatre in Saint Petersburg, June 2008 (F31).
- The Music Development Company production (for CD release) of Daniel Humair (drums) and Damien Varaillon (double bass) performing their improvisation ‘Hommage à John Coltrane’ (F28) recorded Daniel Humair and Damien Varaillon’s performance in the Bal Blomet (Paris), on 18 January 2018 (F31).
</rdfs:comment>
  </owl:ObjectProperty>
  <owl:ObjectProperty rdf:about="R81i_is_recorded_in">
    <rdfs:label xml:lang="en">R81i is recorded in</rdfs:label>
    <skos:notation>R81i</skos:notation>
    <skos:prefLabel xml:lang="en">is recorded in</skos:prefLabel>
    <rdfs:domain rdf:resource="http://iflastandards.info/ns/lrm/lrmoo/F31_Performance"/>
    <rdfs:range rdf:resource="http://iflastandards.info/ns/lrm/lrmoo/F28_Expression_Creation"/>
    <owl:inverseOf rdf:resource="http://iflastandards.info/ns/lrm/lrmoo/R81_recorded"/>
    <rdfs:comment xml:lang="en">Quantification of the inverse property: many to one (0,1:0,n)

Scope note of the inverse property:
This property associates an instance of F28 Expression Creation with an instance of F31 Performance that it records.
This property allows for the documentation of the association that exists between the outcome of an instance of F28 Expression Creation such as a performance recording, and the instance of F31 Performance that it is a recording of. For documenting performances that are more integral and planned parts of an expression creation (such as the recording of a performance solely done for the purpose of audio or video productions), the use of the property P9 consist of (forms part of) is more specific (and appropriate).

Examples of the inverse property:
- The Hyperion production (for CD release) of Angela Hewitt performing the ‘Goldberg Variations’ (F28) recorded Angela Hewitt’s performance of the ‘Goldberg Variations’ in Christuskirche (Berlin) on 14-17 December 2015 (F31).
- The Deutsche Grammophon video production of Verdi’s ‘La Traviata’ from the Salzburg Festival in 2005 (F28) recorded the live performance of ‘La Traviata’ that was staged by Willy Decker, directed by Brian Large and featuring Anna Netrebko and Rolando Villazón (F31).
- The Deutsche Grammophon audio production of Verdi’s ‘La Traviata’ from the Salzburg Festival in 2005 (F28) recorded the live performance of ‘La Traviata’ performed by the Vienna Philharmonic, conducted by Carlo Rizzi featuring Anna Netrebko and Rolando Villazón (F31).
- The Belair production (DVD) produced by François Duplat and directed for video by Denis Calozzi, of Michel Fokine’s choreography and libretto for Stravinsky’s ‘The Firebird’ (F28) recorded the Mariinsky Orchestra and Ballet’s performance of Michel Fokine’s choreography and libretto (choreographic work) for Stravinsky’s ‘The Firebird’, at the Mariinsky Theatre in Saint Petersburg, June 2008 (F31).
- The Music Development Company production (for CD release) of Daniel Humair (drums) and Damien Varaillon (double bass) performing their improvisation ‘Hommage à John Coltrane’ (F28) recorded Daniel Humair and Damien Varaillon’s performance in the Bal Blomet (Paris), on 18 January 2018 (F31).
</rdfs:comment>
  </owl:ObjectProperty>
</rdf:RDF>
